src/PaperTheorems.v
@@ -2,60 +2,48 @@ Require Import Word.
 Require Import Omega.
 Require Import Bool.
 Require Import Pred.
-Require Import DirCache.
 Require Import GenSepN.
 Require Import ListPred.
-Require Import Inode.
 Require Import List ListUtils.
 Require Import Bytes.
-Require Import DirTree.
 Require Import Rec.
 Require Import Arith.
 Require Import FSLayout.
 Require Import Errno.
-Require Import SuperBlock.
 Require Import Lia.
 Require Import FunctionalExtensionality.
-Require Import BFile.
-Require Import DirTreeDef.
-Require Import DirTreeRep.
-Require Import DirTreePred.
-Require Import DirTreeInodes.
-Require Import DirTreeSafe.
-Require Import AsyncFS.
 Require Import DiskSecDef DiskSecAttacker DiskSecVictim.
-Require Import CopyFile.
+(* Require Import CopyFile. *)
 
 Set Implicit Arguments.
-Import AFS.
+
 Import ListNotations.
 
-Definition equivalent_for_principal u d0 bm0 (hm0:hashmap) d1 bm1 hm1:=
+Definition equivalent_for_principal u d0 bm0 d1 bm1 hm:=
   (forall tag, can_access u tag ->
-  equivalent_for tag d0 d1 /\
-  blockmem_equivalent_for tag bm0 bm1) /\
-  hm0 = hm1.
+  equivalent_for tag d0 d1 hm /\
+  blockmem_equivalent_for tag bm0 bm1 hm).
 
 Definition ret_noninterference {T} (p: prog T):=
-  forall u d0 bm0 hm0 d0' bm0' hm0' ret tr0 d1 bm1 hm1,
+  forall u d0 bm0 hm0 d0' bm0' hm0' ret tr0 d1 bm1,
     exec u d0 bm0 hm0 p (Finished d0' bm0' hm0' ret) tr0 ->
-    equivalent_for_principal u d0 bm0 hm0 d1 bm1 hm1 ->
-    exists d1' bm1' hm1' tr1,
-      exec u d1 bm1 hm1 p (Finished d1' bm1' hm1' ret) tr1.
+    equivalent_for_principal u d0 bm0 d1 bm1 hm0 ->
+    exists d1' bm1' tr1,
+      exec u d1 bm1 hm0 p (Finished d1' bm1' hm0' ret) tr1.
 
 Definition equivalent_state_for_principal {T} u (res0 res1: @result T) :=
-  exists d0 bm0 hm0 d1 bm1 hm1,
-    equivalent_for_principal u d0 bm0 hm0 d1 bm1 hm1 /\
-    ((res0 = Crashed d0 bm0 hm0 /\ res1 = Crashed d1 bm1 hm1) \/
-     (res0 = Failed d0 bm0 hm0 /\ res1 = Failed d1 bm1 hm1) \/
-     (exists v0 v1, res0= Finished d0 bm0 hm0 v0 /\ res1 = Finished d1 bm1 hm1 v1)).
+  exists d0 bm0 hm d1 bm1,
+    equivalent_for_principal u d0 bm0 d1 bm1 hm /\
+    ((res0 = Crashed d0 bm0 hm /\ res1 = Crashed d1 bm1 hm) \/
+     (res0 = Failed /\ res1 = Failed) \/
+     (exists v0 v1, res0= Finished d0 bm0 hm v0 /\ res1 = Finished d1 bm1 hm v1)).
 
 Definition state_noninterference {T} (p: prog T):=
-  forall viewer caller d0 bm0 hm0 res0 tr0 d1 bm1 hm1,
+  forall viewer caller d0 bm0 hm0 res0 tr0 d1 bm1,
     exec caller d0 bm0 hm0 p res0 tr0 ->
-    equivalent_for_principal viewer d0 bm0 hm0 d1 bm1 hm1 ->
+    equivalent_for_principal viewer d0 bm0 d1 bm1 hm0 ->
     exists res1 tr1,
-      exec caller d1 bm1 hm1 p res1 tr1 /\
+      exec caller d1 bm1 hm0 p res1 tr1 /\
       equivalent_state_for_principal viewer res0 res1.
 
 Definition unseal_safe {T} (p:prog T) :=
@@ -67,7 +55,7 @@ Definition unseal_safe {T} (p:prog T) :=
 Definition op_public op:=
   match op with
   | Uns t => t = Public
-  | _ => True
+  | Chd t _ => t = Public
   end.
 
 Definition unseal_public {T} (p:prog T) :=
@@ -139,134 +127,100 @@ Proof.
   eapply exec_equivalent_for_viewer in H0 as Hx; eauto.
   repeat split_ors; cleanup.
   do 2 eexists; repeat split; eauto.
-  do 6 eexists; split.
+  do 5 eexists; split.
   2: { right; right; repeat eexists; eauto. }
-  split; auto.
-  intros t Ht; intuition eauto.
-
+  split; eauto.
+  
   do 2 eexists; repeat split; eauto.
-  do 6 eexists; split.
+  do 5 eexists; split.
   2: { left; repeat eexists; eauto. }
-  split; auto.
+  split; eauto.
 
   do 2 eexists; repeat split; eauto.
-  do 6 eexists; split.
+  do 5 eexists; split.
   2: { right; left; repeat eexists; eauto. }
-  split; auto.
+  split; eauto.
 
+  edestruct H1; eauto.
+  edestruct H1; eauto.
   intros t Ht; specialize (H1 t Ht); intuition.
   intros t Ht; specialize (H1 t Ht); intuition.
 Qed.
 
-
-Theorem write_confidentiality:
-forall caller d bm hm Fr fsxp ds mscs sm Fm Ftop tree ilist frees pathname inum f Fd vs d1 bm1 hm1 r1 tr1 off data0 data1, 
-  (Fr * [[sync_invariant Fr]] *
-   LOG.rep (FSXPLog fsxp) (SB.rep fsxp) (LOG.NoTxn ds) (MSLL mscs) sm bm hm *
-   [[[ ds!! ::: (Fm * rep fsxp Ftop tree ilist frees mscs sm) ]]] *
-   [[ find_subtree pathname tree = Some (TreeFile inum f) ]] *
-   [[[ (DFData f) ::: (Fd * off |-> vs) ]]])%pred d ->
-  exec caller d bm hm (update_fblock_d fsxp inum off data0 mscs) (Finished d1 bm1 hm1 r1) tr1 ->
-  DFOwner f <> Public ->
-  exists d2 bm2 hm2 tr2 r2,
-    exec caller d bm hm (update_fblock_d fsxp inum off data1 mscs) (Finished d2 bm2 hm2 r2) tr2 /\
-  (forall adv, ~can_access adv (DFOwner f) -> equivalent_for_principal adv d1 bm1 hm1 d2 bm2 hm2).
+Theorem chdom_equivalent_for_viewer :
+  forall viewer caller d bm hm d' bm' d1 bm1 hm1 r1 tr1 domid new_tag,
+  exec caller d bm hm (ChDom domid new_tag) (Finished d1 bm1 hm1 r1) tr1 ->
+  equivalent_for_principal viewer d bm d' bm' hm ->
+  (same_for_domainid domid d bm d' bm' \/ ~can_access viewer new_tag) ->
+  
+   exists d2 bm2 tr2,
+     exec caller d' bm' hm (ChDom domid new_tag) (Finished d2 bm2 hm1 r1) tr2 /\
+     equivalent_for_principal viewer d1 bm1 d2 bm2 hm1 /\
+     (same_for_domainid domid d bm d' bm' -> same_for_domainid domid d1 bm1 d2 bm2) /\
+     (~can_access viewer new_tag -> equivalent_for_principal viewer d1 bm1 d2 bm2 hm).
 Proof.
-  unfold update_fblock_d; intros.
+  intros.
   inv_exec_perm.
-  pose proof (@update_fblock_d'_ok fsxp inum off mscs caller) as Hspec.
-  specialize (Hspec _ (fun r => Ret r)).
-  unfold corr2 in *.
-  edestruct Hspec with (d:= d).
-  Opaque update_fblock_d'.
-  2: repeat econstructor; eauto.
+  do 3 eexists; split; eauto.
+  econstructor; eauto.
+  split; eauto.
+  unfold equivalent_for_principal in *; eauto.
+  intros; eauto.
+  specialize (H0 _ H).
+  split_ors.
   {
-    repeat eexists; pred_apply; cancel.
-    eauto.
-    eauto.
-    destruct_lift H4.
-    inv_exec'' H7.
-    left; repeat eexists; eauto.
-    eassign (fun (d:rawdisk) (bm' :block_mem) (hm': hashmap) (r: BFILE.memstate * (res tag * unit)) =>
-               let mscs' := fst r in let ok := fst (snd r) in
-               (Fr * [[ sync_invariant Fr ]] *LOG.rep (FSXPLog fsxp) (SB.rep fsxp) (LOG.ActiveTxn ds ds!!) (MSLL mscs') sm bm' hm' *
-               [[[ ds!! ::: (Fm * rep fsxp Ftop tree ilist (frees_1, frees_2) mscs' sm) ]]] *
-               [[ find_subtree pathname tree = Some (TreeFile inum f) ]] *
-               [[[ (DFData f) ::: (Fd * off |-> vs) ]]] *     
-               ([[ isError ok ]] \/
-                exists t, [[ ok = OK t ]] * [[ t = DFOwner f ]] * [[ can_access caller t ]]))%pred d); simpl ;auto.
-    pred_apply; cancel.
-    or_l; cancel.
-    or_r; cancel.
-    inv_exec'' H7; simpl; auto.
-    eassign (fun (_:block_mem) (_: hashmap) (_:rawdisk) => True); simpl;
-      intros mx Hmx; simpl; auto.
-  }
-  simpl in *; clear Hspec; split_ors; cleanup; try congruence.
-  eapply exec_same_except_finished in H0; eauto; cleanup.
-  unfold pair_args_helper in *; simpl in *.
-  apply sep_star_or_distr in H5; apply pimpl_or_apply in H5;
-    split_ors; destruct_lift H5; cleanup.
-  inversion H9.
-  {
-    Transparent LOG.commit_ro LOG.abort.
-    unfold LOG.abort in *.
-    repeat inv_exec_perm.
-    do 5 eexists; split.
-    econstructor; eauto.
-    inversion H19; subst.
-    simpl; rewrite <- app_nil_l; repeat econstructor; eauto.
-    repeat split; simpl; eauto.
-    destruct (tag_dec tag (DFOwner f)); subst; intuition.
-    eapply same_except_to_equivalent_for; eauto.
-    destruct (tag_dec tag (DFOwner f)); subst; intuition.
-    eapply blockmem_same_except_to_equivalent_for; eauto.
-  }
-  {
-    inversion H9; subst.
-    Transparent LOG.commit_ro LOG.abort.
-    unfold LOG.commit_ro in *.
-    repeat inv_exec_perm.
-    inversion H22; subst.
-    specialize (H6 x8) as Hx; split_ors; cleanup; try congruence.
-    pose proof (@DIRTREE.dwrite_ok fsxp inum off x8 x8_1 caller) as Hspec.
-    specialize (Hspec _ (fun r => Ret r)).
-    unfold corr2 in *.
-    edestruct Hspec with (d:= x9).
-    Opaque DIRTREE.dwrite.
-    2: repeat econstructor; eauto.
+    split.
     {
-      repeat eexists; pred_apply; norm.
-      unfold stars; simpl.
-      erewrite LOG.rep_blockmem_subset. cancel.
-      eauto.
-      intuition eauto.
-      apply Mem.upd_eq; eauto.
-      simpl; auto.
-      destruct_lift H2.
-      inv_exec'' H9.
-      left; repeat eexists; eauto.
-      eassign (fun (_:rawdisk) (_:block_mem) (_: hashmap) (_: BFILE.memstate) => True); simpl ;auto.
-      inv_exec'' H9; simpl; auto.
-      eassign (fun (_:block_mem) (_: hashmap) (_:rawdisk) => True); simpl;
-        intros mx Hmx; simpl; auto.
+      unfold equivalent_for, same_for_domainid, same_for_domainid_disk in *; intros.
+      specialize (H0 a); split_ors; cleanup; eauto.
+      specialize (H1 a _ _ H0 H4).
+      right; do 2 eexists; repeat split; eauto.
+      eapply forall_forall2.      
+      apply forall2_forall in H5.
+      apply forall2_forall in H6.
+      apply forall2_forall in H1.
+      rewrite Forall_forall in *; intros.
+      destruct (addr_eq_dec domid (fst (fst x1))).
+      eapply H1; eauto.
+      erewrite <- H5; eauto.
+      rewrite Mem.upd_ne in H8; eauto.
+      eapply forall2_length; eauto.
     }
-    simpl in *; clear H2 Hspec.
-    eapply exec_same_except_finished with (bm':=(Mem.upd x2 x8 (DFOwner f, data1)))in H8;
-    eauto; cleanup.
-    do 5 eexists; split.
-    repeat econstructor; eauto.
-    simpl; repeat econstructor; eauto.
-    repeat split; simpl; eauto.
-    destruct (tag_dec tag (DFOwner f)); subst; intuition.
-    eapply same_except_to_equivalent_for; eauto.
-    destruct (tag_dec tag (DFOwner f)); subst; intuition.
-    eapply blockmem_same_except_to_equivalent_for; eauto.
-    eapply blockmem_same_except_upd_same; eauto.
-    apply only_public_operations_impl; auto.
+    {
+      unfold blockmem_equivalent_for, same_for_domainid, same_for_domainid_mem in *; intros.
+      specialize (H2 a); split_ors; cleanup; eauto.
+      specialize (H3 a _ _ H2 H4).
+      right; do 2 eexists; repeat split; eauto.
+      intros; destruct (addr_eq_dec domid (fst x)).
+      eapply H3; eauto.
+      erewrite <- H5; eauto.
+      rewrite Mem.upd_ne in H7; eauto.
+    }
   }
-  congruence.
-  apply same_except_refl.
-  apply blockmem_same_except_refl.
-  apply only_public_operations_impl; auto.
+  {
+    destruct (tag_dec tag new_tag); subst; intuition.
+    {
+      unfold equivalent_for in *; intros.
+      specialize (H0 a); split_ors; cleanup; eauto.
+      right; do 2 eexists; repeat split; eauto.
+      eapply forall_forall2.      
+      apply forall2_forall in H4.
+      apply forall2_forall in H5.
+      rewrite Forall_forall in *; intros.
+      destruct (addr_eq_dec domid (fst (fst x1))); subst.
+      rewrite Mem.upd_eq in H7; eauto.
+      cleanup; congruence.
+      rewrite Mem.upd_ne in H7; eauto.
+      eapply forall2_length; eauto.
+    }
+    {
+      unfold blockmem_equivalent_for in *; intros.
+      specialize (H2 a); split_ors; cleanup; eauto.
+      right; do 2 eexists; repeat split; eauto.
+      intros; destruct (addr_eq_dec domid (fst x)); subst.
+      rewrite Mem.upd_eq in H6; eauto.
+      cleanup; congruence.
+      rewrite Mem.upd_ne in H6; eauto.
+    }
+  }
 Qed.
