src/ChownNoninterference.v
@@ -1,0 +1,1353 @@
+Require Import Arith.
+Require Import Mem Pred.
+Require Import Word.
+Require Import Omega.
+Require Import List ListUtils.
+Require Import Bool.
+Require Import Eqdep_dec.
+Require Import Setoid.
+Require Import Rec.
+Require Import FunctionalExtensionality.
+Require Import NArith.
+Require Import WordAuto.
+Require Import Errno.
+
+Require Import GenSepAuto. 
+Require Import ListPred.
+Require Import Log.
+Require Import Balloc.
+Require Import FSLayout.
+Require Import BlockPtr.
+Require Import Inode BFile DirTree.
+Require Import DiskSecAttacker PaperTheorems.
+Import INODE.
+
+
+
+    Opaque IRec.get_array IRec.put_array.
+    Theorem inode_setowner_exec_equivalent_cant_access:
+  forall viewer caller d bm hm d' bm' Fr lxp xp bxp Fi Fs IFs ino m0 m ms cache sm Fm ilist inum F d1 bm1 hm1 r1 tr1 new_tag,
+    
+  (Fr * [[sync_invariant Fr]] * [[ hm 0 = Some Public ]] *
+   LOG.rep lxp F (LOG.ActiveTxn m0 m) ms sm bm hm *
+   [[[ m ::: (Fm * rep bxp IFs xp ilist cache hm) ]]] *
+   [[[ ilist ::: (Fi * inum |-> ino) ]]] *
+   [[ (Fs * IFs)%pred sm ]] *
+   [[ can_access caller (IOwner ino) ]])%pred d ->
+  
+  exec caller d bm hm (setowner lxp xp inum new_tag cache ms) (Finished d1 bm1 hm1 r1) tr1 ->
+  equivalent_for_principal viewer d bm d' bm' hm ->
+  ~can_access viewer new_tag ->
+  exists d2 bm2 tr2,
+    exec caller d' bm' hm (setowner lxp xp inum new_tag cache ms) (Finished d2 bm2 hm1 r1) tr2 /\
+    equivalent_for_principal viewer d1 bm1 d2 bm2 hm1 /\
+    equivalent_for_principal viewer d1 bm1 d2 bm2 hm.
+    Proof.
+       unfold setowner, equivalent_for_principal; intros.
+       inv_exec_perm.
+       pose proof (@IRec.get_array_ok lxp xp inum cache ms caller) as Hspec.
+       specialize (Hspec _ (fun r => Ret r)).
+       unfold corr2 in *.
+       unfold rep in *; destruct_lift H.
+       edestruct Hspec with (d:= d).
+       2: repeat econstructor; eauto.
+       { (** extract postcondition from LOG.begin **)
+         clear Hspec; 
+         repeat eexists; pred_apply; cancel.
+         denote listmatch as Hm;
+           rewrite listmatch_length_pimpl in Hm.
+         destruct_lift Hm.
+         rewrite combine_length_eq in *; eauto.
+         denote (length _ = length _) as Hlen;
+           setoid_rewrite <- Hlen.
+         eapply list2nmem_inbound; eauto.
+        match goal with
+           [H: context [ donec = _ ] |- _ ] =>
+           rename H into Hpc;
+          instantiate (2:= fun (d:rawdisk) (bm' :taggedmem) (hm': domainmem)
+                    (r: IRec.Cache_type * (LOG.mstate * cachestate * (IRec.LRA.Defs.item * unit))) =>
+                    let cache' := fst r in let ms' := fst (snd r) in let ret := fst (snd (snd r)) in
+                    (Fr * [[ hm = hm' ]] *
+                    LOG.rep lxp F (LOG.ActiveTxn m0 m) ms' sm bm' hm' *
+                    [[ ((listmatch (inode_match bxp) (combine ilist dummy0) dummy ✶ Fm) *
+                        IRec.rep xp dummy cache')%pred (list2nmem m) ]] *
+                    [[ ret = selN dummy inum IRec.LRA.Defs.item0 ]])%pred d) in Hpc
+        end.
+         destruct_lift Hpc.
+         denote Ret as Hret; inv_exec'' Hret.
+         do 3 eexists; left; repeat eexists; eauto.
+          simpl ;auto.
+         pred_apply; cancel.
+         denote Ret as Hret; inv_exec'' Hret; simpl; auto.
+         eassign (fun (_:taggedmem) (_: domainmem) (_:rawdisk) => True); simpl;
+           intros mx Hmx; simpl; auto.
+       }
+       simpl in *; clear Hspec; cleanup; split_ors; cleanup; try congruence.
+       eapply exec_equivalent_for_viewer_finished in H0; eauto; cleanup.
+       2: intros; edestruct H1; eauto.
+       2: intros; edestruct H1; eauto.
+       unfold pair_args_helper in *; simpl in *.
+
+       destruct_lifts.
+       inv_exec_perm.
+        pose proof (@IRec.put_array_ok lxp xp inum ^( x1_2_2_1_1,
+            ^( ^( x1, x7_1, x7_2_1, x7_2_2_1, x7_2_2_2_1, x7_2_2_2_2_1, x7_2_2_2_2_2_1, x7_2_2_2_2_2_2_1),
+            encode_tag new_tag, x8_2_1), x9_1, x9_2_1, x9_2_2_1, x9_2_2_2_1) x1_1 
+            (x1_2_1_1, x1_2_1_2) caller) as Hspec.
+       specialize (Hspec _ (fun r => Ret r)).
+       unfold corr2 in *.
+       destruct_lifts.
+       edestruct Hspec with (d:= x5).
+       2: repeat econstructor; eauto.
+       { (** extract postcondition from LOG.begin **)
+         clear Hspec; 
+           repeat eexists; pred_apply; cancel; eauto.
+         irec_wf.
+         
+         denote listmatch as Hm;
+           rewrite listmatch_length_pimpl in Hm.
+         destruct_lift Hm.
+         rewrite combine_length_eq in *; [ |eauto].
+         sepauto.
+         match goal with
+           [H: context [ donec = _ ] |- _ ] =>
+           rename H into Hpc;
+           instantiate (2:= fun (d:rawdisk) (bm' :taggedmem) (hm': domainmem)
+                    (r: IRec.Cache_type * (LOG.mstate * cachestate *  unit)) =>
+                    let cache' := fst r in let ms' := fst (snd r) in
+                    let e := ^( x1_2_2_1_1,
+               ^( ^( x1, x7_1, x7_2_1, x7_2_2_1, x7_2_2_2_1, x7_2_2_2_2_1, x7_2_2_2_2_2_1, x7_2_2_2_2_2_2_1),
+               encode_tag new_tag, x8_2_1), x9_1, x9_2_1, x9_2_2_1, x9_2_2_2_1) in
+                    let items' := dummy ⟦ inum := e ⟧ in
+                    exists m',
+                    (Fr * [[ x7 = hm' ]] *
+                    LOG.rep lxp F (LOG.ActiveTxn m0 m') ms' sm bm' hm' *
+                    [[[ m' ::: (Fm ✶ listmatch (inode_match bxp) (combine ilist dummy0) dummy)
+                        * IRec.rep xp items' cache' ]]] *
+                    [[[ items' ::: (arrayN_ex (ptsto (V:=IRec.LRA.Defs.item)) dummy inum) * (inum |-> e) ]]])%pred d) in Hpc
+         end.
+         destruct_lift Hpc.
+         denote Ret as Hret; inv_exec'' Hret.
+         do 3 eexists; left; repeat eexists; eauto.
+         
+         simpl ;auto.
+         pred_apply; cancel.
+         denote Ret as Hret; inv_exec'' Hret; simpl; auto.
+         eassign (fun (_:taggedmem) (_: domainmem) (_:rawdisk) => True); simpl;
+           intros mx Hmx; simpl; auto.
+       }
+       simpl in *; clear Hspec; cleanup; split_ors; cleanup; try congruence.
+       eapply exec_equivalent_for_viewer_finished in H3; eauto; cleanup.
+       unfold pair_args_helper in *; simpl in *.
+
+       inv_exec_perm.
+       denote ChDom as Hdom; eapply chdom_equivalent_for_viewer in Hdom; eauto.
+       2: unfold equivalent_for_principal; intuition eauto.
+       simpl in *; cleanup; try congruence.
+       inv_exec_perm.
+       denote (_ = _) as Heq; inversion Heq; subst; clear Heq.
+       do 3 eexists; split; eauto.
+       repeat (econstructor; [eauto| simpl]);
+         econstructor; eauto.
+       split; eauto.
+       denote lift_empty as Hemp; destruct_lift Hemp; eauto.
+       unfold equivalent_for_principal in *; eauto.
+
+       Unshelve.
+       all: try exact addr; try exact nil; try exact IRec.LRA.Defs.item0; eauto.
+    Qed.
+    
+    Theorem inode_setowner_exec_equivalent_same_for_id:
+  forall viewer caller d bm hm d' bm' Fr lxp xp bxp Fi Fs IFs ino m0 m ms cache sm Fm ilist inum F d1 bm1 hm1 r1 tr1 new_tag,
+    
+  (Fr * [[sync_invariant Fr]] * [[ hm 0 = Some Public ]] *
+   LOG.rep lxp F (LOG.ActiveTxn m0 m) ms sm bm hm *
+   [[[ m ::: (Fm * rep bxp IFs xp ilist cache hm) ]]] *
+   [[[ ilist ::: (Fi * inum |-> ino) ]]] *
+   [[ (Fs * IFs)%pred sm ]] *
+   [[ can_access caller (IOwner ino) ]])%pred d ->
+  
+  exec caller d bm hm (setowner lxp xp inum new_tag cache ms) (Finished d1 bm1 hm1 r1) tr1 ->
+  equivalent_for_principal viewer d bm d' bm' hm ->
+  same_for_domainid (S inum) d bm d' bm' ->
+  exists d2 bm2 tr2,
+    exec caller d' bm' hm (setowner lxp xp inum new_tag cache ms) (Finished d2 bm2 hm1 r1) tr2 /\
+    equivalent_for_principal viewer d1 bm1 d2 bm2 hm1 /\
+    same_for_domainid (S inum) d1 bm1 d2 bm2.
+    Proof.
+      unfold setowner, equivalent_for_principal; intros.
+       inv_exec_perm.
+       pose proof (@IRec.get_array_ok lxp xp inum cache ms caller) as Hspec.
+       specialize (Hspec _ (fun r => Ret r)).
+       unfold corr2 in *.
+       unfold rep in *; destruct_lift H.
+       edestruct Hspec with (d:= d).
+       2: repeat econstructor; eauto.
+       { (** extract postcondition from LOG.begin **)
+         clear Hspec; 
+         repeat eexists; pred_apply; cancel.
+         denote listmatch as Hm;
+           rewrite listmatch_length_pimpl in Hm.
+         destruct_lift Hm.
+         rewrite combine_length_eq in *; eauto.
+         denote (length _ = length _) as Hlen;
+           setoid_rewrite <- Hlen.
+         eapply list2nmem_inbound; eauto.
+         match goal with
+           [H: context [ donec = _ ] |- _ ] =>
+           rename H into Hpc;
+          instantiate (2:= fun (d:rawdisk) (bm' :taggedmem) (hm': domainmem)
+                    (r: IRec.Cache_type * (LOG.mstate * cachestate * (IRec.LRA.Defs.item * unit))) =>
+                    let cache' := fst r in let ms' := fst (snd r) in let ret := fst (snd (snd r)) in
+                    (Fr * [[ hm = hm' ]] *
+                    LOG.rep lxp F (LOG.ActiveTxn m0 m) ms' sm bm' hm' *
+                    [[ ((listmatch (inode_match bxp) (combine ilist dummy0) dummy ✶ Fm) *
+                        IRec.rep xp dummy cache')%pred (list2nmem m) ]] *
+                    [[ ret = selN dummy inum IRec.LRA.Defs.item0 ]])%pred d) in Hpc
+        end.
+         destruct_lift Hpc.
+         denote Ret as Hret; inv_exec'' Hret.
+         do 3 eexists; left; repeat eexists; eauto.
+         simpl ;auto.
+         pred_apply; cancel.
+         denote Ret as Hret; inv_exec'' Hret; simpl; auto.
+         eassign (fun (_:taggedmem) (_: domainmem) (_:rawdisk) => True); simpl;
+           intros mx Hmx; simpl; auto.
+       }
+       simpl in *; clear Hspec; cleanup; split_ors; cleanup; try congruence.
+       eapply exec_equivalent_for_viewer_same_for_domain_id_finished in H0; eauto; cleanup.
+       2: intros; edestruct H1; eauto.
+       2: intros; edestruct H1; eauto.
+       unfold pair_args_helper in *; simpl in *.
+       
+       destruct_lifts.
+       inv_exec_perm.
+        pose proof (@IRec.put_array_ok lxp xp inum ^( x1_2_2_1_1,
+            ^( ^( x1, x7_1, x7_2_1, x7_2_2_1, x7_2_2_2_1, x7_2_2_2_2_1, x7_2_2_2_2_2_1, x7_2_2_2_2_2_2_1),
+            encode_tag new_tag, x8_2_1), x9_1, x9_2_1, x9_2_2_1, x9_2_2_2_1) x1_1 
+            (x1_2_1_1, x1_2_1_2) caller) as Hspec.
+       specialize (Hspec _ (fun r => Ret r)).
+       unfold corr2 in *.
+       destruct_lifts.
+       edestruct Hspec with (d:= x5).
+       2: repeat econstructor; eauto.
+       { (** extract postcondition from LOG.begin **)
+         clear Hspec; 
+           repeat eexists; pred_apply; cancel; eauto.
+         irec_wf.
+         
+         denote listmatch as Hm;
+           rewrite listmatch_length_pimpl in Hm.
+         destruct_lift Hm.
+         rewrite combine_length_eq in *; [ |eauto].
+         sepauto.
+         match goal with
+           [H: context [ donec = _ ] |- _ ] =>
+           rename H into Hpc;
+           instantiate (2:= fun (d:rawdisk) (bm' :taggedmem) (hm': domainmem)
+                    (r: IRec.Cache_type * (LOG.mstate * cachestate *  unit)) =>
+                    let cache' := fst r in let ms' := fst (snd r) in
+                    let e := ^( x1_2_2_1_1,
+               ^( ^( x1, x7_1, x7_2_1, x7_2_2_1, x7_2_2_2_1, x7_2_2_2_2_1, x7_2_2_2_2_2_1, x7_2_2_2_2_2_2_1),
+               encode_tag new_tag, x8_2_1), x9_1, x9_2_1, x9_2_2_1, x9_2_2_2_1) in
+                    let items' := dummy ⟦ inum := e ⟧ in
+                    exists m',
+                    (Fr * [[ x7 = hm' ]] *
+                    LOG.rep lxp F (LOG.ActiveTxn m0 m') ms' sm bm' hm' *
+                    [[[ m' ::: (Fm ✶ listmatch (inode_match bxp) (combine ilist dummy0) dummy)
+                        * IRec.rep xp items' cache' ]]] *
+                    [[[ items' ::: (arrayN_ex (ptsto (V:=IRec.LRA.Defs.item)) dummy inum) * (inum |-> e) ]]])%pred d) in Hpc
+         end.
+         destruct_lift Hpc.
+         denote Ret as Hret; inv_exec'' Hret.
+         do 3 eexists; left; repeat eexists; eauto.
+         simpl ;auto.
+         pred_apply; cancel.
+         denote Ret as Hret; inv_exec'' Hret; simpl; auto.
+         eassign (fun (_:taggedmem) (_: domainmem) (_:rawdisk) => True); simpl;
+           intros mx Hmx; simpl; auto.
+       }
+       simpl in *; clear Hspec; cleanup; split_ors; cleanup; try congruence.
+       eapply exec_equivalent_for_viewer_same_for_domain_id_finished in H3; eauto; cleanup.
+       unfold pair_args_helper in *; simpl in *.
+
+       inv_exec_perm.
+       denote ChDom as Hdom; eapply chdom_equivalent_for_viewer in Hdom; eauto.
+       2: unfold equivalent_for_principal; intuition eauto.
+       simpl in *; cleanup; try congruence.
+       inv_exec_perm.
+       denote (_ = _) as Heq; inversion Heq; subst; clear Heq.
+       do 3 eexists; split; eauto.
+       repeat (econstructor; [eauto| simpl]);
+         econstructor; eauto.
+
+       Unshelve.
+       all: try exact addr; try exact nil; try exact IRec.LRA.Defs.item0; eauto.
+    Qed.
+
+
+    Import BFILE.
+    Theorem bfile_setowner_exec_equivalent_cant_access:
+  forall viewer caller d bm hm d' bm' Fr Ff f bxps lxp ixp allocc frees flist m0 m ms sm Fm ilist inum F d1 bm1 hm1 r1 tr1 new_tag,
+    
+  (Fr * [[sync_invariant Fr]] * [[ hm 0 = Some Public ]] *
+  LOG.rep lxp F (LOG.ActiveTxn m0 m) (MSLL ms) sm bm hm *
+  [[[ m ::: (Fm * rep bxps sm ixp flist ilist frees allocc (MSCache ms) (MSICache ms) (MSDBlocks ms) hm) ]]] *
+  [[[ flist ::: (Ff * inum |-> f) ]]] *
+  [[ can_access caller (BFOwner f) ]])%pred d ->
+  
+  exec caller d bm hm (setowner lxp ixp inum new_tag ms) (Finished d1 bm1 hm1 r1) tr1 ->
+  equivalent_for_principal viewer d bm d' bm' hm ->
+  ~can_access viewer new_tag ->
+  exists d2 bm2 tr2,
+    exec caller d' bm' hm (setowner lxp ixp inum new_tag ms) (Finished d2 bm2 hm1 r1) tr2 /\
+    equivalent_for_principal viewer d1 bm1 d2 bm2 hm1 /\
+    equivalent_for_principal viewer d1 bm1 d2 bm2 hm.
+    Proof.
+      unfold setowner; intros.
+      inv_exec_perm.
+      unfold rep in *.
+      destruct_lift H.
+      eapply inode_setowner_exec_equivalent_cant_access in H0; eauto.
+      cleanup.
+      unfold pair_args_helper in *; simpl in *.
+      inv_exec_perm.
+      do 3 eexists; split; eauto.
+       repeat (econstructor; [eauto| simpl]);
+         econstructor; eauto.
+      pred_apply; cancel.
+      sepauto.
+
+      denote listmatch as Hx;
+        rewrite listmatch_length_pimpl in Hx.
+      destruct_lift Hx.
+      assert (A:inum < length flist). { eapply list2nmem_inbound; eauto. }
+      assert (A0:inum < length ilist). { match goal with [H: length _ = ?x |- _ < ?x ] => rewrite <- H; eauto end. }
+      denote listmatch as Hx.
+      rewrite listmatch_isolate with (i:=inum) in Hx by auto.
+      unfold file_match in Hx; destruct_lift Hx.
+      rewrite <- H21; eauto.
+      erewrite <- list2nmem_sel; eauto.
+
+      Unshelve.
+      exact bfile0.
+      Grab Existential Variables.
+      exact inode0.
+    Qed.
+
+
+    Theorem bfile_setowner_exec_equivalent_same_for_id:
+  forall viewer caller d bm hm d' bm' Fr Ff f bxps lxp ixp allocc frees flist m0 m ms sm Fm ilist inum F d1 bm1 hm1 r1 tr1 new_tag,
+    
+  (Fr * [[sync_invariant Fr]] * [[ hm 0 = Some Public ]] *
+  LOG.rep lxp F (LOG.ActiveTxn m0 m) (MSLL ms) sm bm hm *
+  [[[ m ::: (Fm * rep bxps sm ixp flist ilist frees allocc (MSCache ms) (MSICache ms) (MSDBlocks ms) hm) ]]] *
+  [[[ flist ::: (Ff * inum |-> f) ]]] *
+  [[ can_access caller (BFOwner f) ]])%pred d ->
+  
+  exec caller d bm hm (setowner lxp ixp inum new_tag ms) (Finished d1 bm1 hm1 r1) tr1 ->
+  equivalent_for_principal viewer d bm d' bm' hm ->
+  same_for_domainid (S inum) d bm d' bm' ->
+  exists d2 bm2 tr2,
+    exec caller d' bm' hm (setowner lxp ixp inum new_tag ms) (Finished d2 bm2 hm1 r1) tr2 /\
+    equivalent_for_principal viewer d1 bm1 d2 bm2 hm1 /\
+    same_for_domainid (S inum) d1 bm1 d2 bm2.
+    Proof.
+      unfold setowner; intros.
+      inv_exec_perm.
+      unfold rep in *.
+      destruct_lift H.
+      eapply inode_setowner_exec_equivalent_same_for_id in H0; eauto.
+      cleanup.
+      unfold pair_args_helper in *; simpl in *.
+      inv_exec_perm.
+      do 3 eexists; split; eauto.
+       repeat (econstructor; [eauto| simpl]);
+         econstructor; eauto.
+      pred_apply; cancel.
+      sepauto.
+
+      denote listmatch as Hx;
+        rewrite listmatch_length_pimpl in Hx.
+      destruct_lift Hx.
+      assert (A:inum < length flist). { eapply list2nmem_inbound; eauto. }
+      assert (A0:inum < length ilist). { match goal with [H: length _ = ?x |- _ < ?x ] => rewrite <- H; eauto end. }
+      denote listmatch as Hx.
+      rewrite listmatch_isolate with (i:=inum) in Hx by auto.
+      unfold file_match in Hx; destruct_lift Hx.
+      rewrite <- H21; eauto.
+      erewrite <- list2nmem_sel; eauto.
+
+      Unshelve.
+      exact bfile0.
+      Grab Existential Variables.
+      exact inode0.
+    Qed.
+
+    Require Import DirTreePath.
+    Require Import DirTreeDef.
+    Require Import DirTreePred.
+    Require Import DirTreeRep.
+    Require Import DirTreeSafe.
+    Require Import DirTreeNames.
+    Require Import DirTreeInodes.
+    Import DIRTREE.
+   
+    Theorem dirtree_changeowner_exec_equivalent_cant_access:
+  forall viewer caller d bm hm d' bm' Fr f fsxp frees m0 m mscs sm Fm ilist inum F d1 bm1 hm1 r1 tr1 new_tag tree Ftop pathname,
+    
+  (Fr * [[sync_invariant Fr]] * [[ hm 0 = Some Public ]] *
+  LOG.rep (FSXPLog fsxp) F (LOG.ActiveTxn m0 m) (MSLL mscs) sm bm hm *
+  [[ (Fm * rep fsxp Ftop tree ilist frees mscs sm hm)%pred (list2nmem m) ]] *
+  [[ find_subtree pathname tree = Some (TreeFile inum f) ]] *
+  [[ can_access caller (DFOwner f) ]])%pred d ->
+  
+  exec caller d bm hm (changeowner fsxp inum new_tag mscs) (Finished d1 bm1 hm1 r1) tr1 ->
+  equivalent_for_principal viewer d bm d' bm' hm ->
+  ~can_access viewer new_tag ->
+  exists d2 bm2 tr2,
+    exec caller d' bm' hm (changeowner fsxp inum new_tag mscs) (Finished d2 bm2 hm1 r1) tr2 /\
+    equivalent_for_principal viewer d1 bm1 d2 bm2 hm1 /\
+    equivalent_for_principal viewer d1 bm1 d2 bm2 hm.
+    Proof.
+       unfold changeowner; intros.
+       inv_exec_perm.
+      unfold rep in *.
+      destruct_lift H.
+      rewrite subtree_extract in * by eauto.
+      cbn [tree_pred] in *. destruct_lifts.
+      
+      eapply bfile_setowner_exec_equivalent_cant_access in H0; eauto.
+      cleanup.
+      unfold pair_args_helper in *; simpl in *.
+      inv_exec_perm.
+      do 3 eexists; split; eauto.
+       repeat (econstructor; [eauto| simpl]);
+         econstructor; eauto.
+       pred_apply; cancel.
+    Qed.
+
+
+    Theorem dirtree_changeowner_exec_equivalent_same_for_id:
+  forall viewer caller d bm hm d' bm' Fr f fsxp frees m0 m mscs sm Fm ilist inum F d1 bm1 hm1 r1 tr1 new_tag tree Ftop pathname,
+    
+  (Fr * [[sync_invariant Fr]] * [[ hm 0 = Some Public ]] *
+  LOG.rep (FSXPLog fsxp) F (LOG.ActiveTxn m0 m) (MSLL mscs) sm bm hm *
+  [[ (Fm * rep fsxp Ftop tree ilist frees mscs sm hm)%pred (list2nmem m) ]] *
+  [[ find_subtree pathname tree = Some (TreeFile inum f) ]] *
+  [[ can_access caller (DFOwner f) ]])%pred d ->
+  
+  exec caller d bm hm (changeowner fsxp inum new_tag mscs) (Finished d1 bm1 hm1 r1) tr1 ->
+  equivalent_for_principal viewer d bm d' bm' hm ->
+  same_for_domainid (S inum) d bm d' bm' ->
+  exists d2 bm2 tr2,
+    exec caller d' bm' hm (changeowner fsxp inum new_tag mscs) (Finished d2 bm2 hm1 r1) tr2 /\
+    equivalent_for_principal viewer d1 bm1 d2 bm2 hm1 /\
+    same_for_domainid (S inum) d1 bm1 d2 bm2.
+    Proof.
+      unfold changeowner; intros.
+      inv_exec_perm.
+      unfold rep in *.
+      destruct_lift H.
+      rewrite subtree_extract in * by eauto.
+      cbn [tree_pred] in *. destruct_lifts.
+      
+      eapply bfile_setowner_exec_equivalent_same_for_id in H0; eauto.
+      cleanup.
+      unfold pair_args_helper in *; simpl in *.
+      inv_exec_perm.
+      do 3 eexists; split; eauto.
+       repeat (econstructor; [eauto| simpl]);
+         econstructor; eauto.
+       pred_apply; cancel.
+    Qed.
+
+    Require Import SuperBlock AsyncFS.
+    Import AFS.
+
+    Import DiskSecDef.
+
+  Fixpoint no_domain_change {T} (p: prog T) :=
+    match p with
+    | Bind p1 p2 =>  no_domain_change p1 /\ (forall r, no_domain_change (p2 r))
+    | ChDom _ _ => False
+    | _ => True
+    end.
+
+  Lemma no_domain_change_foreach:
+           forall (ITEM : Type) (lst : list ITEM) (L : Type) (G : Type) (f : ITEM -> L -> prog L)
+                (nocrash : G -> list ITEM -> L -> taggedmem -> domainmem -> rawpred tagged_block)
+                (crashed : G -> taggedmem -> domainmem -> rawpred tagged_block) (l : L),
+          (forall i l, no_domain_change (f i l)) ->
+          no_domain_change (ForEach_ f lst nocrash crashed l).
+        Proof.
+          induction lst; simpl; eauto.
+        Qed.
+
+        Lemma no_domain_change_forn:
+           forall n i (L : Type) (G : Type) (f : nat -> L -> prog L)
+                (nocrash : G -> nat -> L -> taggedmem -> domainmem -> rawpred tagged_block)
+                (crashed : G -> taggedmem -> domainmem -> rawpred tagged_block) (l : L),
+          (forall i l, no_domain_change (f i l)) ->
+          no_domain_change (ForN_ f i n nocrash crashed l).
+        Proof.
+          induction n; simpl; eauto.
+        Qed.
+        
+      Ltac delve :=
+        match goal with
+        | [ |- context [ If (?x) { _ } else { _ }] ] =>
+          let D := fresh "D" in
+          destruct x eqn:D; try setoid_rewrite D; simpl; repeat split; intros; eauto; clear D; repeat delve
+        | [ |- context [ match ?x with | _ =>  _ end ] ] =>
+          let D := fresh "D" in
+          destruct x eqn:D; try setoid_rewrite D; simpl; repeat split; intros; eauto; clear D; repeat delve
+        | [ |- context [ let _ := ?x in _ ] ] =>
+          destruct x; simpl; repeat split; intros; eauto; repeat delve
+        | [ |- no_domain_change (ForEach_ _ _ _ _ _) ] =>
+          eapply no_domain_change_foreach; eauto; intros; simpl; repeat split; intros; eauto; repeat delve
+        | [ |- no_domain_change (ForN_ _ _ _ _ _ _) ] =>
+          eapply no_domain_change_forn; eauto; intros; simpl; repeat split; intros; eauto; repeat delve
+        end.
+
+        
+        
+      Lemma no_domain_change_commit:
+        forall a b,
+          no_domain_change (LOG.commit a b).
+      Proof.
+        intros.
+        Transparent LOG.commit.
+        unfold LOG.commit, GLog.submit, GLog.flushall_noop,
+        GLog.flushall, GLog.flushall_nomerge, pair_args_helper; simpl.
+        unfold avail, extend, MLog.flush, MLog.apply, MLog.flush_noapply,
+        DiskLogPadded.avail, DiskLogPadded.extend, 
+        CacheDef.read, maybe_evict, evict, writeback,
+        pair_args_helper; simpl.
+        delve.
+        all: unfold pair_args_helper; simpl.
+        all: intros; try delve. 
+        all: unfold CacheDef.read; unfold maybe_evict; unfold evict; unfold writeback; simpl; try delve.
+      Qed.
+  
+  Lemma equivalent_no_domain_change_cant_access:
+    forall T (p: prog T) viewer caller d bm d' bm' d1 bm1 hm hm' hm1 i ntg tr1 r1,
+      exec caller d bm hm' p (Finished d1 bm1 hm1 r1) tr1 ->
+      (forall tag, can_access viewer tag -> equivalent_for tag d d' hm) ->
+      (forall tag, can_access viewer tag -> blockmem_equivalent_for tag bm bm' hm) ->
+      only_public_operations tr1 ->
+      ~can_access viewer ntg ->
+      hm' = upd hm i ntg ->
+      no_domain_change p ->
+      exists d2 bm2 tr2,
+        exec caller d' bm' hm' p (Finished d2 bm2 hm1 r1) tr2 /\
+      (forall tag, can_access viewer tag -> equivalent_for tag d1 d2 hm) /\
+      (forall tag, can_access viewer tag -> blockmem_equivalent_for tag bm1 bm2 hm) /\
+      hm' = hm1.
+  Proof.
+    induction p; intros; inv_exec_perm;
+    try solve [do 3 eexists; split; [econstructor; eauto|
+                                     split; eauto ] ].
+  { (** Read **)
+    destruct bs.
+    specialize H1 with (1:= can_access_public viewer) as Hx;
+    specialize (Hx r1); intuition; cleanup; try congruence.
+    specialize H0 with (1:= can_access_public viewer) as Hx;
+    specialize (Hx n); intuition; cleanup; try congruence.
+    destruct x0, t0.
+    unfold vsmerge in *; simpl in *.
+    repeat (denote (Forall2 _ (_::_)(_::_)) as Hf; inversion Hf; clear Hf; subst).
+    do 3 eexists; split.
+    econstructor; eauto.
+    split; eauto.
+    split; eauto.
+    unfold blockmem_equivalent_for; intros.
+    destruct (handle_eq_dec a r1); subst.
+    right.
+    repeat rewrite Mem.upd_eq; eauto.
+    do 2 eexists; eauto.
+    split; eauto.
+    split; eauto.
+    split; eauto.
+    intros.
+    simpl in *; eauto.
+    specialize H0 with (1:= H) as Hx;
+    specialize (Hx n); intuition; cleanup; try congruence.
+    unfold vsmerge in *; simpl in *.
+    repeat (denote (Forall2 _ (_::_)(_::_)) as Hf; inversion Hf; clear Hf; subst).
+    eauto.
+    repeat rewrite Mem.upd_ne; eauto.
+    eapply H1; eauto.
+  }
+  { (** Write **)
+    destruct b, bs, t; simpl in *.
+    destruct (hm n0) eqn: D.    
+    destruct (can_access_dec viewer t).
+    { (** can access **)
+      specialize H0 with (1:= can_access_public viewer) as Hx;
+      specialize (Hx n); intuition; cleanup; try congruence.
+      specialize H1 with (1:= c) as Hx;
+      specialize (Hx h); intuition; cleanup; try congruence.
+      destruct x0, x1; simpl in *; cleanup.
+      do 3 eexists; split.
+      econstructor; eauto.
+      split; eauto.
+      unfold equivalent_for; intros.
+      specialize H0 with (1:= H) as Hx;
+      specialize (Hx n); destruct Hx; cleanup; try congruence.
+      destruct (addr_eq_dec a n); subst.
+      right.
+      repeat rewrite Mem.upd_eq; eauto.
+      do 2 eexists; eauto.
+      split; eauto.
+      split.
+      unfold vsmerge in *; simpl in *; eauto.
+      unfold vsmerge in *; simpl in *; eauto.
+      repeat rewrite Mem.upd_ne; eauto.
+      eapply H0; eauto.
+    }
+    { (** can't access **)
+      specialize H0 with (1:= can_access_public viewer) as Hx;
+      specialize (Hx n); intuition; cleanup; try congruence.
+      specialize H1 with (1:= can_access_public viewer) as Hx;
+      specialize (Hx h); intuition; cleanup; try congruence.
+      destruct x0, x1; simpl in *; cleanup.
+      do 3 eexists; split.
+      econstructor; eauto.
+      split; eauto.
+      unfold equivalent_for; intros.
+      destruct (tag_dec t tag); subst; intuition.
+      specialize H0 with (1:= H) as Hx;
+      specialize (Hx n); destruct Hx; cleanup; try congruence.
+      destruct (addr_eq_dec a n); subst.
+      right.
+      repeat rewrite Mem.upd_eq; eauto.
+      do 2 eexists; eauto.
+      split; eauto.
+      split; eauto.
+      split.
+      unfold vsmerge in *; simpl in *; eauto.
+      unfold vsmerge in *; simpl in *; eauto.
+      econstructor.
+      simpl; intros; cleanup; intuition.
+      eauto.
+      repeat rewrite Mem.upd_ne; eauto.
+      eapply H0; eauto.
+    }
+    { (** inconsistent **)
+      specialize H0 with (1:= can_access_public viewer) as Hx;
+      specialize (Hx n); intuition; cleanup; try congruence.
+      specialize H1 with (1:= can_access_public viewer) as Hx;
+      specialize (Hx h); intuition; cleanup; try congruence.
+      destruct x0, x1; simpl in *; cleanup.
+      do 3 eexists; split.
+      econstructor; eauto.
+      split; eauto.
+      unfold equivalent_for; intros.
+      specialize H0 with (1:= H) as Hx;
+      specialize (Hx n); destruct Hx; cleanup; try congruence.
+      destruct (addr_eq_dec a n); subst.
+      right.
+      repeat rewrite Mem.upd_eq; eauto.
+      do 2 eexists; eauto.
+      split; eauto.
+      split; eauto.
+      split.
+      unfold vsmerge in *; simpl in *; eauto.
+      unfold vsmerge in *; simpl in *; eauto.
+      econstructor.
+      simpl; intros; congruence.
+      eauto.
+      repeat rewrite Mem.upd_ne; eauto.
+      eapply H0; eauto.
+    }
+  }
+  { (** Seal **)
+    specialize H1 with (1:= can_access_public viewer) as Hx;
+    specialize (Hx r1); intuition; cleanup; try congruence.
+    do 3 eexists; split.
+    econstructor; eauto.
+    split; eauto.
+    split; eauto.
+    unfold blockmem_equivalent_for; intros.
+    destruct (handle_eq_dec a r1); subst.
+    right.
+    repeat rewrite Mem.upd_eq; eauto.
+    do 2 eexists; eauto.
+    repeat rewrite Mem.upd_ne; eauto.
+    eapply H1; eauto.
+  }
+  { (** Unseal **)
+    intuition.
+    destruct b; simpl in *.
+    specialize H1 with (1:= can_access_public viewer) as Hx;
+    specialize (Hx h); intuition; cleanup; try congruence.
+    simpl in *; intuition; subst.
+    do 3 eexists; split.
+    rewrite H8.
+    econstructor; eauto.
+    destruct (addr_eq_dec i (fst x0)); subst.
+    rewrite upd_eq in *; eauto.
+    cleanup; intuition.
+    rewrite upd_ne in *; eauto.
+    split; eauto.
+  }
+  { (** Sync **)
+    repeat eexists; [econstructor; eauto| |eauto].
+    unfold equivalent_for in *; intros.
+    specialize H0 with (1:= H) as Hx.
+    unfold sync_mem.
+    specialize (Hx a); split_ors; cleanup; eauto.
+    repeat match goal with
+           | [H: ?x = _ |- context [?x] ] => rewrite H
+           end; eauto.
+    repeat match goal with
+           | [H: ?x = _ |- context [?x] ] => rewrite H
+           end; eauto.
+    destruct x, x0.
+    unfold vsmerge in *; simpl in *; eauto.
+    repeat (denote (Forall2 _ (_::_)(_::_)) as Hf; inversion Hf; clear Hf; subst).
+    right; repeat eexists; simpl; eauto.    
+  }
+  {
+    simpl in *; intuition.
+  }
+  { (** Bind **)
+    apply only_public_operations_app in H3; cleanup.
+    destruct H6.
+    specialize IHp with (1:=H0)(2:=H1)(3:=H2)(4:=H5)(5:=H4); cleanup.
+    edestruct IHp; eauto; cleanup.
+    specialize H with (1:=H7)(2:=H10)(3:=H11)(4:=H3)(5:=H4); cleanup.
+    edestruct H; eauto; cleanup.
+    repeat eexists; [econstructor; eauto| |]; eauto.
+  }
+
+  Unshelve.
+  all: try exact addr; eauto.
+  all: try exact nil.
+  all: try exact eq.
+Qed.
+
+    Theorem changeowner_exec_cant_access:
+  forall viewer caller d bm hm d' bm' Fr fsxp ds mscs sm Fm Ftop tree ilist frees pathname inum f d1 bm1 hm1 r1 tr1 new_tag,
+    
+  (Fr * [[sync_invariant Fr]] * [[ hm 0 = Some Public ]] *
+   LOG.rep (FSXPLog fsxp) (SB.rep fsxp) (LOG.NoTxn ds) (MSLL mscs) sm bm hm *
+   [[[ ds!! ::: (Fm * rep fsxp Ftop tree ilist frees mscs sm hm) ]]] *
+   [[ find_subtree pathname tree = Some (TreeFile inum f) ]])%pred d ->
+
+  exec caller d bm hm (changeowner fsxp inum new_tag mscs) (Finished d1 bm1 hm1 r1) tr1 ->
+  equivalent_for_principal viewer d bm d' bm' hm ->
+  ~can_access viewer new_tag ->
+  exists d2 bm2 tr2,
+    exec caller d' bm' hm (changeowner fsxp inum new_tag mscs) (Finished d2 bm2 hm1 r1) tr2 /\
+    equivalent_for_principal viewer d1 bm1 d2 bm2 hm1.
+Proof.
+  unfold changeowner, equivalent_for_principal; intros.
+  inv_exec_perm.
+  pose proof (@LOG.begin_ok (FSXPLog fsxp) (MSLL mscs) caller) as Hspec.
+  specialize (Hspec _ (fun r => Ret r)).
+  unfold corr2 in *.
+  edestruct Hspec with (d:= d).
+  2: repeat econstructor; eauto.
+  { (** extract postcondition from LOG.begin **)
+    repeat eexists; pred_apply; cancel.
+    match goal with
+           [H: context [ donec = _ ] |- _ ] =>
+           rename H into Hpc;
+          instantiate (2:= fun (d:rawdisk) (bm' :taggedmem) (hm': domainmem) (r: LOG.memstate) =>
+               (Fr * LOG.rep (FSXPLog fsxp) (SB.rep fsxp) (LOG.ActiveTxn ds ds!!) r sm bm' hm' *
+               [[ hm = hm' ]] * [[ LOG.readOnly (MSLL mscs) r ]])%pred d) in Hpc
+        end.
+         destruct_lift Hpc.
+         denote Ret as Hret; inv_exec'' Hret.
+         do 3 eexists; left; repeat eexists; eauto.
+         simpl ;auto.
+         pred_apply; cancel.
+         denote Ret as Hret; inv_exec'' Hret; simpl; auto.
+         eassign (fun (_:taggedmem) (_: domainmem) (_:rawdisk) => True); simpl;
+           intros mx Hmx; simpl; auto.
+  }
+  simpl in *; clear Hspec; cleanup; split_ors; cleanup; try congruence.
+  eapply exec_equivalent_for_viewer_finished in H0; eauto; cleanup.
+  2: intros; edestruct H1; eauto.
+  2: intros; edestruct H1; eauto.
+  unfold pair_args_helper in *; simpl in *.
+
+  denote lift_empty as Hemp; destruct_lift Hemp.
+  denote lift_empty as Hemp; destruct_lift Hemp.
+  inv_exec_perm.
+  pose proof (@DIRTREE.authenticate_ok fsxp inum
+            {|
+            BFILE.MSAlloc := MSAlloc mscs;
+            BFILE.MSLL := (x8_1, x8_2);
+            BFILE.MSAllocC := MSAllocC mscs;
+            BFILE.MSIAllocC := MSIAllocC mscs;
+            BFILE.MSICache := MSICache mscs;
+            BFILE.MSCache := SDIR.MSCache mscs;
+            BFILE.MSDBlocks := MSDBlocks mscs |} caller) as Hspec.
+  specialize (Hspec _ (fun r => Ret r)).
+  unfold corr2 in *.
+  edestruct Hspec with (d:= x5).
+  2: econstructor; eauto; repeat econstructor.
+  { (** extract postcondition from DIRTREE.authenticate **)
+    repeat eexists; pred_apply; cancel.
+    erewrite mscs_same_except_log_rep'.
+    cancel; apply pimpl_refl.
+    unfold BFILE.mscs_same_except_log; simpl; intuition.
+    eauto.
+
+     match goal with
+           [H: context [ donec = _ ] |- _ ] =>
+           rename H into Hpc;
+          instantiate (2:= fun (d:rawdisk) (bm' :taggedmem) (hm': domainmem) (r: BFILE.memstate * (bool * unit)) =>
+               let mscs' := fst r in let ok := fst (snd r) in
+               (Fr * [[ x7 = hm' ]] *
+                LOG.rep (FSXPLog fsxp) (SB.rep fsxp) (LOG.ActiveTxn ds ds!!) (MSLL mscs') sm bm' hm' *
+                [[[ ds!! ::: (Fm * rep fsxp Ftop tree ilist (frees_1, frees_2) mscs' sm hm') ]]] *
+                [[ BFILE.MSAlloc mscs' = BFILE.MSAlloc mscs ]] *
+                [[ BFILE.MSCache mscs' = BFILE.MSCache mscs ]] *
+                [[ MSAllocC mscs' = MSAllocC mscs ]] *
+                [[ MSIAllocC mscs' = MSIAllocC mscs ]] *
+                (([[ ok = true ]] * [[ can_access caller (DFOwner f) ]]) \/
+                 ([[ ok = false ]] * [[ ~can_access caller (DFOwner f) ]])))%pred d) in Hpc
+        end.
+     destruct_lift Hpc.
+     denote Ret as Hret; inv_exec'' Hret.
+      do 3 eexists; left; repeat eexists; eauto.
+      simpl ;auto.
+      pred_apply; cancel.
+      or_l; cancel.
+      or_r; cancel.
+      denote Ret as Hret; inv_exec'' Hret; simpl; auto.
+      eassign (fun (_:taggedmem) (_: domainmem) (_:rawdisk) => True); simpl;
+      intros mx Hmx; simpl; auto.
+  }
+  simpl in *; clear Hspec; cleanup; split_ors; cleanup; try congruence.
+  eapply exec_equivalent_for_viewer_finished in H3; eauto; cleanup.
+  unfold pair_args_helper in *; simpl in *.
+
+  denote lift_empty as Hemp; destruct_lift Hemp.
+  denote or as Hor;
+  apply sep_star_or_distr in Hor; apply pimpl_or_apply in Hor;
+    split_ors; denote lift_empty as Hemp; destruct_lift Hemp; cleanup; simpl in *.
+  { (* DIRTREE.authenticate returns true *)
+    inv_exec_perm.
+    pose proof (@DIRTREE.getowner_ok fsxp inum x15_1 caller) as Hspec.
+    specialize (Hspec _ (fun r => Ret r)).
+    unfold corr2 in *.
+    edestruct Hspec with (d:= x0).
+    2: econstructor; eauto; repeat econstructor.
+    { (** extract postcondition from DIRTREE.getowner **)
+      repeat eexists; pred_apply; cancel.
+      cancel; apply pimpl_refl.
+      eauto.
+
+       match goal with
+           [H: context [ donec = _ ] |- _ ] =>
+           rename H into Hpc;
+          instantiate (2:= fun (d:rawdisk) (bm' :taggedmem) (hm': domainmem) (r: BFILE.memstate * (tag * unit)) =>
+               let mscs' := fst r in let r := fst (snd r) in
+               (Fr * ⟦⟦ x14 = hm' ⟧⟧ *
+                LOG.rep fsxp.(FSXPLog) (SB.rep fsxp) (LOG.ActiveTxn ds ds!!) (MSLL mscs') sm bm' hm' *
+                [[[ ds!! ::: Fm * rep fsxp Ftop tree ilist (frees_1, frees_2) mscs' sm hm' ]]] *
+                [[ BFILE.MSAlloc mscs' = BFILE.MSAlloc mscs ]] *
+                [[ BFILE.MSCache mscs' = BFILE.MSCache mscs ]] *
+                [[ MSAllocC mscs' = MSAllocC mscs ]] *
+                [[ MSIAllocC mscs' = MSIAllocC mscs ]] *
+                [[ r = DFOwner f ]])%pred d) in Hpc
+        end.
+         destruct_lift Hpc.
+         denote Ret as Hret; inv_exec'' Hret.
+         do 3 eexists; left; repeat eexists; eauto.
+         simpl ;auto.
+         pred_apply; cancel.
+         denote Ret as Hret; inv_exec'' Hret; simpl; auto.
+         eassign (fun (_:taggedmem) (_: domainmem) (_:rawdisk) => True); simpl;
+           intros mx Hmx; simpl; auto.
+  }
+  simpl in *; clear Hspec; cleanup; split_ors; cleanup; try congruence.
+  eapply exec_equivalent_for_viewer_finished in H9; eauto; cleanup.
+  unfold pair_args_helper in *; simpl in *.
+
+  denote lift_empty as Hemp; destruct_lift Hemp.
+  inv_exec_perm.
+  pose proof (@DIRTREE.changeowner_ok fsxp inum new_tag x21_1 caller) as Hspec.
+    specialize (Hspec _ (fun r => Ret r)).
+    unfold corr2 in *.
+    edestruct Hspec with (d:= x8).
+    2: econstructor; eauto; repeat econstructor.
+    { (** extract postcondition from DIRTREE.getowner **)
+      repeat eexists; pred_apply; cancel.
+      cancel; apply pimpl_refl.
+      eauto.
+
+       match goal with
+           [H: context [ donec = _ ] |- _ ] =>
+           rename H into Hpc;
+          instantiate (2:=fun (d:rawdisk) (bm' :taggedmem) (hm': domainmem) (r: BFILE.memstate) =>
+               let mscs' := r in
+               exists m' tree' f' ilist',
+                 (Fr *               
+           LOG.rep fsxp.(FSXPLog) (SB.rep fsxp) (LOG.ActiveTxn ds m') (MSLL mscs') sm bm' hm' *
+           [[ (Fm * rep fsxp Ftop tree' ilist' (frees_1, frees_2) mscs' sm hm')%pred (list2nmem m') ]] *
+           [[ tree' = update_subtree pathname (TreeFile inum f') tree ]] *
+           [[ f' = mk_dirfile (DFData f) (DFAttr f) new_tag ]] *
+           [[ MSAlloc mscs' = MSAlloc mscs ]] *
+           [[ dirtree_safe ilist  (BFILE.pick_balloc (frees_1, frees_2)  (MSAlloc mscs')) tree
+                           ilist' (BFILE.pick_balloc (frees_1, frees_2)  (MSAlloc mscs')) tree' ]] *
+           [[ BFILE.treeseq_ilist_safe inum ilist ilist' ]] *
+           [[ hm' = upd x20 (S inum) new_tag ]])%pred d) in Hpc
+        end.
+         destruct_lift Hpc.
+         denote Ret as Hret; inv_exec'' Hret.
+          do 3 eexists; left; repeat eexists; eauto.
+         simpl ;auto.
+         pred_apply; cancel.
+         denote Ret as Hret; inv_exec'' Hret; simpl; auto.
+         eassign (fun (_:taggedmem) (_: domainmem) (_:rawdisk) => True); simpl;
+           intros mx Hmx; simpl; auto.
+  }
+  simpl in *; clear Hspec; cleanup; split_ors; cleanup; try congruence.
+  eapply dirtree_changeowner_exec_equivalent_cant_access in H18; eauto.
+  3: unfold equivalent_for_principal; intuition eauto.
+  2: {
+    pred_apply; safecancel.
+    cancel; apply pimpl_refl.
+    eauto.
+    eauto.
+  }
+  cleanup.
+  
+  denote lift_empty as Hemp; destruct_lift Hemp.
+  inv_exec_perm.
+  pose proof (@LOG.commit_ok (FSXPLog fsxp) (AFS.MSLL x27) caller) as Hspec.
+  specialize (Hspec _ (fun r => Ret r)).
+  unfold corr2 in *.
+  edestruct Hspec with (d:= x12).
+  2: econstructor; eauto; repeat econstructor.
+  { (** extract postcondition from LOG.begin **)
+    repeat eexists; pred_apply; cancel.
+    
+     match goal with
+       [H: context [ donec = _ ] |- _ ] =>
+       rename H into Hpc;
+         instantiate (2:= fun (d:rawdisk) (bm' :taggedmem) (hm': domainmem) (r: LOG.memstate * (bool * unit)) =>
+           let ms' := fst r in let r := fst (snd r) in
+             (Fr * ⟦⟦ (upd x20 (S inum) new_tag) = hm' ⟧⟧ *
+              (([[ r = true ]] *  LOG.rep (FSXPLog fsxp) (SB.rep fsxp)  (LOG.NoTxn (pushd x28 ds)) ms' sm bm' hm') \/
+               ([[ r = false ]] *
+                [[ MapUtils.AddrMap.Map.cardinal (LOG.MSTxn (fst (AFS.MSLL x27))) > (LogLen (FSXPLog fsxp)) ]] *
+                LOG.rep (FSXPLog fsxp) (SB.rep fsxp)  (LOG.NoTxn ds) ms' sm bm' hm')))%pred d) in Hpc
+        end.
+         destruct_lift Hpc.
+         denote Ret as Hret; inv_exec'' Hret.
+    
+         do 3 eexists; left; repeat eexists; eauto.
+         simpl ;auto.
+         pred_apply; cancel.
+         or_l; cancel.
+         or_r; cancel.
+         denote Ret as Hret; inv_exec'' Hret; simpl; auto.
+         eassign (fun (_:taggedmem) (_: domainmem) (_:rawdisk) => True); simpl;
+           intros mx Hmx; simpl; auto.
+  }
+  simpl in *; clear Hspec; cleanup; split_ors; cleanup; try congruence.
+   denote lift_empty as Hemp; destruct_lift Hemp.
+  denote or as Hor;
+  apply sep_star_or_distr in Hor; apply pimpl_or_apply in Hor;
+    split_ors; denote lift_empty as Hemp; 
+      destruct_lift Hemp; cleanup; simpl in *.
+  {
+    eapply exec_equivalent_for_viewer_finished in H29; eauto; cleanup.
+    2: intros; edestruct H31; eauto.
+    2: intros; edestruct H31; eauto.
+    unfold pair_args_helper in *; simpl in *.
+    inv_exec_perm.
+    denote (_ = _) as Heq; inversion Heq; subst; clear Heq.
+
+    do 3 eexists; split; eauto.
+    econstructor; [eauto| simpl].
+    econstructor; [eauto| simpl].
+    econstructor; [eauto| simpl].
+    econstructor; [eauto| simpl].
+    econstructor; [eauto| simpl].
+    econstructor; eauto.
+  }
+  
+  {
+    eapply equivalent_no_domain_change_cant_access in H29; eauto; cleanup.
+    unfold pair_args_helper in *; simpl in *.    
+    inv_exec_perm.
+    inv_exec_perm.    
+    denote (_ = _) as Heq; inversion Heq; subst; clear Heq.
+    inv_exec_perm.
+    
+    do 3 eexists; split; eauto.
+    econstructor; [eauto| simpl].
+    econstructor; [eauto| simpl].
+    econstructor; [eauto| simpl].
+    econstructor; [eauto| simpl].
+    econstructor; [eauto| simpl].
+    econstructor; [eauto| simpl].  
+    econstructor; eauto.
+    econstructor; eauto.
+    rewrite upd_repeat, upd_nop; eauto.
+    unfold rep in H8; destruct_lift H8.
+    erewrite owner_match; eauto.
+    2: pred_apply' H8; cancel.
+    2: pred_apply; cancel.
+    denote tree_pred as Htp; erewrite subtree_extract in Htp; eauto.
+    unfold tree_pred in Htp; destruct_lift Htp.    
+    denote BFILE.rep as Hbf; unfold BFILE.rep in Hbf; destruct_lift Hbf.
+    denote listmatch as Hlm;
+       erewrite listmatch_length_pimpl in Hlm;
+      erewrite listmatch_isolate with (i:=inum) in Hlm.
+    unfold file_match in Hlm.
+    destruct_lift Hlm.
+    denote INODE.rep as Hbf; unfold INODE.rep in Hbf; destruct_lift Hbf.
+    rewrite H64; apply H69.
+    rewrite <- H62.
+    eapply list2nmem_ptsto_bound; eauto; pred_apply; cancel.
+    eapply list2nmem_ptsto_bound; eauto; pred_apply; cancel.
+    destruct_lift Hlm.
+    rewrite <- H62; eapply list2nmem_ptsto_bound; eauto; pred_apply; cancel.
+    intros; edestruct H38; eauto.
+    intros; edestruct H38; eauto.
+    apply no_domain_change_commit.      
+  }
+  }
+  { (** auth returned false **)
+    Transparent LOG.abort.
+    unfold LOG.abort in *.
+    inv_exec_perm.
+    inv_exec_perm.    
+    denote (_ = _) as Heq; inversion Heq; subst; clear Heq.
+    inv_exec_perm.    
+    denote (_ = _) as Heq; inversion Heq; subst; clear Heq.
+    rewrite H18.
+    do 3 eexists; split; eauto.
+    econstructor; [eauto| simpl].
+    econstructor; [eauto| simpl].
+    econstructor; [eauto| simpl].
+    econstructor; eauto.
+    rewrite <- H18; econstructor; eauto.
+  }
+
+  Unshelve.
+  all: try exact addr; eauto.
+Qed.
+
+
+
+
+  Theorem changeowner_exec_same_for_id:
+  forall viewer caller d bm hm d' bm' Fr fsxp ds mscs sm Fm Ftop tree ilist frees pathname inum f d1 bm1 hm1 r1 tr1 new_tag,
+    
+  (Fr * [[sync_invariant Fr]] * [[ hm 0 = Some Public ]] *
+   LOG.rep (FSXPLog fsxp) (SB.rep fsxp) (LOG.NoTxn ds) (MSLL mscs) sm bm hm *
+   [[[ ds!! ::: (Fm * rep fsxp Ftop tree ilist frees mscs sm hm) ]]] *
+   [[ find_subtree pathname tree = Some (TreeFile inum f) ]])%pred d ->
+
+  exec caller d bm hm (changeowner fsxp inum new_tag mscs) (Finished d1 bm1 hm1 r1) tr1 ->
+  equivalent_for_principal viewer d bm d' bm' hm ->
+  same_for_domainid (S inum) d bm d' bm' ->
+  exists d2 bm2 tr2,
+    exec caller d' bm' hm (changeowner fsxp inum new_tag mscs) (Finished d2 bm2 hm1 r1) tr2 /\
+    equivalent_for_principal viewer d1 bm1 d2 bm2 hm1.
+Proof.
+  unfold changeowner, equivalent_for_principal; intros.
+  inv_exec_perm.
+  pose proof (@LOG.begin_ok (FSXPLog fsxp) (MSLL mscs) caller) as Hspec.
+  specialize (Hspec _ (fun r => Ret r)).
+  unfold corr2 in *.
+  edestruct Hspec with (d:= d).
+  2: repeat econstructor; eauto.
+  { (** extract postcondition from LOG.begin **)
+    repeat eexists; pred_apply; cancel.
+    match goal with
+           [H: context [ donec = _ ] |- _ ] =>
+           rename H into Hpc;
+          instantiate (2:= fun (d:rawdisk) (bm' :taggedmem) (hm': domainmem) (r: LOG.memstate) =>
+               (Fr * LOG.rep (FSXPLog fsxp) (SB.rep fsxp) (LOG.ActiveTxn ds ds!!) r sm bm' hm' *
+               [[ hm = hm' ]] * [[ LOG.readOnly (MSLL mscs) r ]])%pred d) in Hpc
+        end.
+         destruct_lift Hpc.
+         denote Ret as Hret; inv_exec'' Hret.
+         do 3 eexists; left; repeat eexists; eauto.
+         simpl ;auto.
+         pred_apply; cancel.
+         denote Ret as Hret; inv_exec'' Hret; simpl; auto.
+         eassign (fun (_:taggedmem) (_: domainmem) (_:rawdisk) => True); simpl;
+           intros mx Hmx; simpl; auto.
+  }
+  simpl in *; clear Hspec; cleanup; split_ors; cleanup; try congruence.
+  eapply exec_equivalent_for_viewer_same_for_domain_id_finished in H0; eauto; cleanup.
+  2: intros; edestruct H1; eauto.
+  2: intros; edestruct H1; eauto.
+  unfold pair_args_helper in *; simpl in *.
+
+  denote lift_empty as Hemp; destruct_lift Hemp.
+  denote lift_empty as Hemp; destruct_lift Hemp.
+  inv_exec_perm.
+  pose proof (@DIRTREE.authenticate_ok fsxp inum
+            {|
+            BFILE.MSAlloc := MSAlloc mscs;
+            BFILE.MSLL := (x8_1, x8_2);
+            BFILE.MSAllocC := MSAllocC mscs;
+            BFILE.MSIAllocC := MSIAllocC mscs;
+            BFILE.MSICache := MSICache mscs;
+            BFILE.MSCache := SDIR.MSCache mscs;
+            BFILE.MSDBlocks := MSDBlocks mscs |} caller) as Hspec.
+  specialize (Hspec _ (fun r => Ret r)).
+  unfold corr2 in *.
+  edestruct Hspec with (d:= x5).
+  2: econstructor; eauto; repeat econstructor.
+  { (** extract postcondition from DIRTREE.authenticate **)
+    repeat eexists; pred_apply; cancel.
+    erewrite mscs_same_except_log_rep'.
+    cancel; apply pimpl_refl.
+    unfold BFILE.mscs_same_except_log; simpl; intuition.
+    eauto.
+
+     match goal with
+           [H: context [ donec = _ ] |- _ ] =>
+           rename H into Hpc;
+          instantiate (2:= fun (d:rawdisk) (bm' :taggedmem) (hm': domainmem) (r: BFILE.memstate * (bool * unit)) =>
+               let mscs' := fst r in let ok := fst (snd r) in
+               (Fr * [[ x7 = hm' ]] *
+                LOG.rep (FSXPLog fsxp) (SB.rep fsxp) (LOG.ActiveTxn ds ds!!) (MSLL mscs') sm bm' hm' *
+                [[[ ds!! ::: (Fm * rep fsxp Ftop tree ilist (frees_1, frees_2) mscs' sm hm') ]]] *
+                [[ BFILE.MSAlloc mscs' = BFILE.MSAlloc mscs ]] *
+                [[ BFILE.MSCache mscs' = BFILE.MSCache mscs ]] *
+                [[ MSAllocC mscs' = MSAllocC mscs ]] *
+                [[ MSIAllocC mscs' = MSIAllocC mscs ]] *
+                (([[ ok = true ]] * [[ can_access caller (DFOwner f) ]]) \/
+                 ([[ ok = false ]] * [[ ~can_access caller (DFOwner f) ]])))%pred d) in Hpc
+        end.
+     destruct_lift Hpc.
+     denote Ret as Hret; inv_exec'' Hret.
+      do 3 eexists; left; repeat eexists; eauto.
+      simpl ;auto.
+      pred_apply; cancel.
+      or_l; cancel.
+      or_r; cancel.
+      denote Ret as Hret; inv_exec'' Hret; simpl; auto.
+      eassign (fun (_:taggedmem) (_: domainmem) (_:rawdisk) => True); simpl;
+      intros mx Hmx; simpl; auto.
+  }
+  simpl in *; clear Hspec; cleanup; split_ors; cleanup; try congruence.
+  eapply exec_equivalent_for_viewer_same_for_domain_id_finished in H3; eauto; cleanup.
+  unfold pair_args_helper in *; simpl in *.
+
+  denote lift_empty as Hemp; destruct_lift Hemp.
+  denote or as Hor;
+  apply sep_star_or_distr in Hor; apply pimpl_or_apply in Hor;
+    split_ors; denote lift_empty as Hemp; destruct_lift Hemp; cleanup; simpl in *.
+  { (* DIRTREE.authenticate returns true *)
+    inv_exec_perm.
+    pose proof (@DIRTREE.getowner_ok fsxp inum x15_1 caller) as Hspec.
+    specialize (Hspec _ (fun r => Ret r)).
+    unfold corr2 in *.
+    edestruct Hspec with (d:= x0).
+    2: econstructor; eauto; repeat econstructor.
+    { (** extract postcondition from DIRTREE.getowner **)
+      repeat eexists; pred_apply; cancel.
+      cancel; apply pimpl_refl.
+      eauto.
+
+       match goal with
+           [H: context [ donec = _ ] |- _ ] =>
+           rename H into Hpc;
+          instantiate (2:= fun (d:rawdisk) (bm' :taggedmem) (hm': domainmem) (r: BFILE.memstate * (tag * unit)) =>
+               let mscs' := fst r in let r := fst (snd r) in
+               (Fr * ⟦⟦ x14 = hm' ⟧⟧ *
+                LOG.rep fsxp.(FSXPLog) (SB.rep fsxp) (LOG.ActiveTxn ds ds!!) (MSLL mscs') sm bm' hm' *
+                [[[ ds!! ::: Fm * rep fsxp Ftop tree ilist (frees_1, frees_2) mscs' sm hm' ]]] *
+                [[ BFILE.MSAlloc mscs' = BFILE.MSAlloc mscs ]] *
+                [[ BFILE.MSCache mscs' = BFILE.MSCache mscs ]] *
+                [[ MSAllocC mscs' = MSAllocC mscs ]] *
+                [[ MSIAllocC mscs' = MSIAllocC mscs ]] *
+                [[ r = DFOwner f ]])%pred d) in Hpc
+        end.
+         destruct_lift Hpc.
+         denote Ret as Hret; inv_exec'' Hret.
+         do 3 eexists; left; repeat eexists; eauto.
+         simpl ;auto.
+         pred_apply; cancel.
+         denote Ret as Hret; inv_exec'' Hret; simpl; auto.
+         eassign (fun (_:taggedmem) (_: domainmem) (_:rawdisk) => True); simpl;
+           intros mx Hmx; simpl; auto.
+  }
+  simpl in *; clear Hspec; cleanup; split_ors; cleanup; try congruence.
+  eapply exec_equivalent_for_viewer_same_for_domain_id_finished in H10; eauto; cleanup.
+  unfold pair_args_helper in *; simpl in *.
+
+  denote lift_empty as Hemp; destruct_lift Hemp.
+  inv_exec_perm.
+  pose proof (@DIRTREE.changeowner_ok fsxp inum new_tag x21_1 caller) as Hspec.
+    specialize (Hspec _ (fun r => Ret r)).
+    unfold corr2 in *.
+    edestruct Hspec with (d:= x8).
+    2: econstructor; eauto; repeat econstructor.
+    { (** extract postcondition from DIRTREE.getowner **)
+      repeat eexists; pred_apply; cancel.
+      cancel; apply pimpl_refl.
+      eauto.
+
+       match goal with
+           [H: context [ donec = _ ] |- _ ] =>
+           rename H into Hpc;
+          instantiate (2:=fun (d:rawdisk) (bm' :taggedmem) (hm': domainmem) (r: BFILE.memstate) =>
+               let mscs' := r in
+               exists m' tree' f' ilist',
+                 (Fr *               
+           LOG.rep fsxp.(FSXPLog) (SB.rep fsxp) (LOG.ActiveTxn ds m') (MSLL mscs') sm bm' hm' *
+           [[ (Fm * rep fsxp Ftop tree' ilist' (frees_1, frees_2) mscs' sm hm')%pred (list2nmem m') ]] *
+           [[ tree' = update_subtree pathname (TreeFile inum f') tree ]] *
+           [[ f' = mk_dirfile (DFData f) (DFAttr f) new_tag ]] *
+           [[ MSAlloc mscs' = MSAlloc mscs ]] *
+           [[ dirtree_safe ilist  (BFILE.pick_balloc (frees_1, frees_2)  (MSAlloc mscs')) tree
+                           ilist' (BFILE.pick_balloc (frees_1, frees_2)  (MSAlloc mscs')) tree' ]] *
+           [[ BFILE.treeseq_ilist_safe inum ilist ilist' ]] *
+           [[ hm' = upd x20 (S inum) new_tag ]])%pred d) in Hpc
+        end.
+         destruct_lift Hpc.
+         denote Ret as Hret; inv_exec'' Hret.
+          do 3 eexists; left; repeat eexists; eauto.
+         simpl ;auto.
+         pred_apply; cancel.
+         denote Ret as Hret; inv_exec'' Hret; simpl; auto.
+         eassign (fun (_:taggedmem) (_: domainmem) (_:rawdisk) => True); simpl;
+           intros mx Hmx; simpl; auto.
+  }
+  simpl in *; clear Hspec; cleanup; split_ors; cleanup; try congruence.
+  eapply dirtree_changeowner_exec_equivalent_same_for_id in H20; eauto.
+  3: unfold equivalent_for_principal; intuition eauto.
+  2: {
+    pred_apply; safecancel.
+    cancel; apply pimpl_refl.
+    eauto.
+    eauto.
+  }
+  cleanup.
+  
+  denote lift_empty as Hemp; destruct_lift Hemp.
+  inv_exec_perm.
+  pose proof (@LOG.commit_ok (FSXPLog fsxp) (AFS.MSLL x27) caller) as Hspec.
+  specialize (Hspec _ (fun r => Ret r)).
+  unfold corr2 in *.
+  edestruct Hspec with (d:= x12).
+  2: econstructor; eauto; repeat econstructor.
+  { (** extract postcondition from LOG.begin **)
+    repeat eexists; pred_apply; cancel.
+    
+     match goal with
+       [H: context [ donec = _ ] |- _ ] =>
+       rename H into Hpc;
+         instantiate (2:= fun (d:rawdisk) (bm' :taggedmem) (hm': domainmem) (r: LOG.memstate * (bool * unit)) =>
+           let ms' := fst r in let r := fst (snd r) in
+             (Fr * ⟦⟦ (upd x20 (S inum) new_tag) = hm' ⟧⟧ *
+              (([[ r = true ]] *  LOG.rep (FSXPLog fsxp) (SB.rep fsxp)  (LOG.NoTxn (pushd x28 ds)) ms' sm bm' hm') \/
+               ([[ r = false ]] *
+                [[ MapUtils.AddrMap.Map.cardinal (LOG.MSTxn (fst (AFS.MSLL x27))) > (LogLen (FSXPLog fsxp)) ]] *
+                LOG.rep (FSXPLog fsxp) (SB.rep fsxp)  (LOG.NoTxn ds) ms' sm bm' hm')))%pred d) in Hpc
+        end.
+         destruct_lift Hpc.
+         denote Ret as Hret; inv_exec'' Hret.
+    
+         do 3 eexists; left; repeat eexists; eauto.
+         simpl ;auto.
+         pred_apply; cancel.
+         or_l; cancel.
+         or_r; cancel.
+         denote Ret as Hret; inv_exec'' Hret; simpl; auto.
+         eassign (fun (_:taggedmem) (_: domainmem) (_:rawdisk) => True); simpl;
+           intros mx Hmx; simpl; auto.
+  }
+  simpl in *; clear Hspec; cleanup; split_ors; cleanup; try congruence.
+   denote lift_empty as Hemp; destruct_lift Hemp.
+  denote or as Hor;
+  apply sep_star_or_distr in Hor; apply pimpl_or_apply in Hor;
+    split_ors; denote lift_empty as Hemp; 
+      destruct_lift Hemp; cleanup; simpl in *.
+  {
+    eapply exec_equivalent_for_viewer_same_for_domain_id_finished in H32; eauto; cleanup.
+    2: intros; edestruct H34; eauto.
+    2: intros; edestruct H34; eauto.
+    unfold pair_args_helper in *; simpl in *.
+    inv_exec_perm.
+    denote (_ = _) as Heq; inversion Heq; subst; clear Heq.
+
+    do 3 eexists; split; eauto.
+    econstructor; [eauto| simpl].
+    econstructor; [eauto| simpl].
+    econstructor; [eauto| simpl].
+    econstructor; [eauto| simpl].
+    econstructor; [eauto| simpl].
+    econstructor; eauto.
+  }
+  
+  {
+    eapply exec_equivalent_for_viewer_same_for_domain_id_finished in H32; eauto; cleanup.
+    2: intros; edestruct H34; eauto.
+    2: intros; edestruct H34; eauto.
+    unfold pair_args_helper in *; simpl in *.    
+    inv_exec_perm.
+    eapply chdom_equivalent_for_viewer in H42; eauto.
+    cleanup.
+    inv_exec_perm.    
+    denote (_ = _) as Heq; inversion Heq; subst; clear Heq.
+
+    do 3 eexists; split; eauto.
+    econstructor; [eauto| simpl].
+    econstructor; [eauto| simpl].
+    econstructor; [eauto| simpl].
+    econstructor; [eauto| simpl].
+    econstructor; [eauto| simpl].
+    econstructor; [eauto| simpl].  
+    econstructor; eauto.
+    unfold equivalent_for_principal; intuition eauto.    
+  }
+  }
+  { (** auth returned false **)
+    Transparent LOG.abort.
+    unfold LOG.abort in *.
+    inv_exec_perm.
+    inv_exec_perm.    
+    denote (_ = _) as Heq; inversion Heq; subst; clear Heq.
+    inv_exec_perm.    
+    denote (_ = _) as Heq; inversion Heq; subst; clear Heq.
+    rewrite H20.
+    do 3 eexists; split; eauto.
+    econstructor; [eauto| simpl].
+    econstructor; [eauto| simpl].
+    econstructor; [eauto| simpl].
+    econstructor; eauto.
+    rewrite <- H20; econstructor; eauto.
+  }
+
+  Unshelve.
+  all: try exact addr; eauto.
+Qed.
+
+Theorem changeowner_state_invariant:
+  forall viewer caller d bm hm d' bm' Fr fsxp ds mscs sm Fm Ftop tree ilist frees pathname inum f d1 bm1 hm1 r1 tr1 new_tag,
+    
+  (Fr * [[sync_invariant Fr]] * [[ hm 0 = Some Public ]] *
+   LOG.rep (FSXPLog fsxp) (SB.rep fsxp) (LOG.NoTxn ds) (MSLL mscs) sm bm hm *
+   [[[ ds!! ::: (Fm * rep fsxp Ftop tree ilist frees mscs sm hm) ]]] *
+   [[ find_subtree pathname tree = Some (TreeFile inum f) ]])%pred d ->
+
+  exec caller d bm hm (changeowner fsxp inum new_tag mscs) (Finished d1 bm1 hm1 r1) tr1 ->
+  equivalent_for_principal viewer d bm d' bm' hm ->
+  (same_for_domainid (S inum) d bm d' bm' \/ ~can_access viewer new_tag) ->
+  exists d2 bm2 tr2,
+    exec caller d' bm' hm (changeowner fsxp inum new_tag mscs) (Finished d2 bm2 hm1 r1) tr2 /\
+    equivalent_for_principal viewer d1 bm1 d2 bm2 hm1.
+Proof.
+  intros.
+  split_ors.
+  eapply changeowner_exec_same_for_id; eauto.
+  eapply changeowner_exec_cant_access; eauto.
+Qed.
