src/HoareWeak.v
@@ -39,11 +39,11 @@ Notation "'{<W' e1 .. e2 , 'PERM' : pr 'PRE' : bm , hm , pre 'POST' : bm' , hm' 
      [[ sync_invariant F_ ]] *
      [[ forall r_ , corr2_weak pr
         (fun done'_ crash'_ bm' hm' =>
-           post F_ r_ * [[ @subset addr addr_eq_dec _ hm hm' ]] *
+           post F_ r_ * [[ hm = hm' ]] *
            [[ bm c= bm' ]] *
            [[ done'_ = done_ ]] * [[ crash'_ = crash_ ]])
         (rx r_) ]] *
-     [[ forall bm'' hm'' , (F_ * crash * [[ @subset addr addr_eq_dec _ hm hm'' ]] *
+     [[ forall bm'' hm'' , (F_ * crash * [[ hm = hm'' ]] *
                        [[ bm c= bm'' ]] ) =p=> crash_ bm'' hm'' ]]
      )) .. ))
    )%pred
@@ -62,10 +62,10 @@ Notation "'{<W' 'PERM' : pr 'PRE' : bm , hm , pre 'POST' : bm' , hm' , post 'CRA
      [[ sync_invariant F_ ]] *
      [[ forall r_ , corr2_weak pr
         (fun done'_ crash'_ bm' hm' =>
-           post F_ r_ * [[ @subset addr addr_eq_dec _ hm hm' ]] *
+           post F_ r_ * [[ hm = hm' ]] *
            [[ bm c= bm' ]] * [[ done'_ = done_ ]] * [[ crash'_ = crash_ ]])
         (rx r_) ]] *
-     [[ forall bm'' hm'' , (F_ * crash * [[ @subset addr addr_eq_dec _ hm hm'' ]] *
+     [[ forall bm'' hm'' , (F_ * crash * [[ hm = hm'' ]] *
                       [[ bm c= bm'' ]]) =p=> crash_ bm'' hm'' ]]
    )%pred
    (Bind p1 rx)%pred)
@@ -103,10 +103,10 @@ Notation "'{!<W' e1 .. e2 , 'PERM' : pr 'PRE' : bm , hm , pre 'POST' : bm' , hm'
      pre *
      [[ forall r_ , corr2_weak pr
         (fun done'_ crash'_ bm' hm' =>
-           post emp r_ * [[ @subset addr addr_eq_dec _ hm hm' ]] *
+           post emp r_ * [[ hm = hm' ]] *
            [[ bm c= bm' ]] * [[ done'_ = done_ ]] * [[ crash'_ = crash_ ]])
         (rx r_) ]] *
-     [[ forall bm'' hm'' , (crash * [[ @subset addr addr_eq_dec _ hm hm'' ]] *
+     [[ forall bm'' hm'' , (crash * [[ hm = hm'' ]] *
                       [[ bm c= bm'' ]]) =p=> crash_ bm'' hm'' ]]
      )) .. ))
    )%pred
@@ -143,10 +143,10 @@ Notation "'{!<W' 'PERM' : pr 'PRE' : bm , hm , pre 'POST' : bm' , hm' , post 'CR
      pre *
      [[ forall r_ , corr2_weak pr
         (fun done'_ crash'_ bm' hm' =>
-           post emp r_ * [[ @subset addr addr_eq_dec _ hm hm' ]] *
+           post emp r_ * [[ hm = hm' ]] *
            [[ bm c= bm' ]] * [[ done'_ = done_ ]] * [[ crash'_ = crash_ ]])
         (rx r_) ]] *
-     [[ forall bm'' hm'' , (crash * [[ @subset addr addr_eq_dec _ hm hm'' ]] *
+     [[ forall bm'' hm'' , (crash * [[ hm = hm'' ]] *
                       [[ bm c= bm'' ]]) =p=> crash_ bm'' hm'' ]]
    )%pred
    (Bind p1 rx)%pred)
@@ -164,12 +164,12 @@ Notation "'{<W' e1 .. e2 , 'PERM' : pr 'PRE' : bm , hm , pre 'POST' : bm' , hm' 
      [[ forall r_ , corr2_weak pr
         (fun done'_ crash'_ bm' hm' =>
            post F_ r_ *
-           [[ bm c= bm' ]] * [[ @subset addr addr_eq_dec _ hm hm' ]] *
+           [[ bm c= bm' ]] * [[ hm = hm' ]] *
            [[ done'_ = done_ ]] * [[ crash'_ = crash_ ]])
         (rx r_) ]] *
      [[ forall realcrash bm'' hm'',
           crash_xform realcrash =p=> crash_xform crash ->
-          (F_ * realcrash * [[ @subset addr addr_eq_dec _ hm hm'' ]] *
+          (F_ * realcrash * [[ hm = hm'' ]] *
                        [[ bm c= bm'' ]] ) =p=> crash_ bm'' hm'' ]]
      )) .. ))
    )%pred
@@ -189,12 +189,12 @@ Notation "'{!<W' e1 .. e2 , 'PERM' : pr 'PRE' : bm , hm , pre 'POST' : bm' , hm'
      [[ forall r_ , corr2_weak pr
         (fun done'_ crash'_ bm' hm' =>
            post F_ r_ *
-           [[ bm c= bm' ]] * [[ @subset addr addr_eq_dec _ hm hm' ]] *
+           [[ bm c= bm' ]] * [[ hm = hm' ]] *
            [[ done'_ = done_ ]] * [[ crash'_ = crash_ ]])
         (rx r_) ]] *
      [[ forall realcrash bm'' hm'',
           crash_xform realcrash =p=> crash_xform crash ->
-          (F_ * realcrash * [[ @subset addr addr_eq_dec _ hm hm'' ]] *
+          (F_ * realcrash * [[ hm = hm'' ]] *
                        [[ bm c= bm'' ]] ) =p=> crash_ bm'' hm'' ]]
      )) .. ))
    )%pred
@@ -335,7 +335,7 @@ Notation "'{W<<' e1 .. e2 , 'PERM' : pr 'PRE' : bm , hm , pre 'POST' : bm' , hm'
      [[ sync_invariant F_ ]] *
      [[ crash_xform F_ =p=> F_ ]] *
      [[ forall r_,
-        {{W pr | fun done'_ crash'_ bm' hm' => post F_ r_ * [[ @subset addr addr_eq_dec _ hm hm' ]] *
+        {{W pr | fun done'_ crash'_ bm' hm' => post F_ r_ * [[ hm = hm' ]] *
           [[ done'_ = done_ ]] *
           [[ bm c= bm' ]] *
           [[ forall bm_crash hm_crash,
@@ -370,7 +370,7 @@ Notation "'{WX<<' e1 .. e2 , 'PERM' : pr 'PRE' : bm , hm , pre 'POST' : bm' , hm
      [[ sync_invariant F_ ]] *
      [[ crash_xform F_ =p=> F_ ]] *
      [[ forall r_,
-        {{W pr | fun done'_ crash'_ bm' hm' => post F_ r_ * [[ @subset addr addr_eq_dec _ hm hm' ]] *
+        {{W pr | fun done'_ crash'_ bm' hm' => post F_ r_ * [[ hm = hm' ]] *
           [[ done'_ = done_ ]] *
           [[ bm c= bm' ]]
         W}} rxOK r_ ]] *
