src/WriteConfidentiality.v
@@ -1,0 +1,165 @@
+Require Import Word.
+Require Import Omega.
+Require Import Bool.
+Require Import Pred.
+Require Import DirCache.
+Require Import GenSepN.
+Require Import ListPred.
+Require Import Inode.
+Require Import List ListUtils.
+Require Import Bytes.
+Require Import DirTree.
+Require Import Rec.
+Require Import Arith.
+Require Import FSLayout.
+Require Import Errno.
+Require Import SuperBlock.
+Require Import Lia.
+Require Import FunctionalExtensionality.
+Require Import BFile.
+Require Import DirTreeDef.
+Require Import DirTreeRep.
+Require Import DirTreePred.
+Require Import DirTreeInodes.
+Require Import DirTreeSafe.
+Require Import AsyncFS.
+Require Import DiskSecDef DiskSecAttacker DiskSecVictim PaperTheorems.
+(* Require Import CopyFile. *)
+Import AFS.
+
+
+
+Theorem write_confidentiality:
+forall caller d bm hm Fr fsxp ds mscs sm Fm Ftop tree ilist frees pathname inum f Fd vs d1 bm1 hm1 r1 tr1 off data0 data1, 
+  (Fr * [[sync_invariant Fr]] * [[ hm 0 = Some Public ]] *
+   LOG.rep (FSXPLog fsxp) (SB.rep fsxp) (LOG.NoTxn ds) (MSLL mscs) sm bm hm *
+   [[[ ds!! ::: (Fm * rep fsxp Ftop tree ilist frees mscs sm hm) ]]] *
+   [[ find_subtree pathname tree = Some (TreeFile inum f) ]] *
+   [[[ (DFData f) ::: (Fd * off |-> vs) ]]])%pred d ->
+  exec caller d bm hm (update_fblock_d fsxp inum off data0 mscs) (Finished d1 bm1 hm1 r1) tr1 ->
+  DFOwner f <> Public ->
+  exists d2 bm2 tr2 r2,
+    exec caller d bm hm (update_fblock_d fsxp inum off data1 mscs) (Finished d2 bm2 hm1 r2) tr2 /\
+  (forall adv, ~can_access adv (DFOwner f) -> equivalent_for_principal adv d1 bm1 d2 bm2 hm1).
+Proof.
+  unfold update_fblock_d; intros.
+  inv_exec_perm.
+  pose proof (@update_fblock_d'_ok fsxp inum off mscs caller) as Hspec.
+  specialize (Hspec _ (fun r => Ret r)).
+  unfold corr2 in *.
+  edestruct Hspec with (d:= d).
+  Opaque update_fblock_d'.
+  2: repeat econstructor; eauto.
+  {
+    repeat eexists; pred_apply; cancel.
+    cancel; eauto.
+    eauto.
+    eauto.
+    destruct_lift H3.
+    inv_exec'' H7.
+    do 3 eexists; left; repeat eexists; eauto.
+    eassign (fun (d:rawdisk) (bm' :taggedmem) (hm': domainmem) (r: BFILE.memstate * (res unit * unit)) =>
+               let mscs' := fst r in let ok := fst (snd r) in
+                (Fr * [[ sync_invariant Fr ]] * [[ hm' 0 = Some Public ]] *
+                 LOG.rep (FSXPLog fsxp) (SB.rep fsxp) (LOG.ActiveTxn ds ds!!) (MSLL mscs') sm bm' hm' *
+               [[[ ds!! ::: (Fm * rep fsxp Ftop tree ilist (frees_1, frees_2) mscs' sm hm') ]]] *
+               [[ find_subtree pathname tree = Some (TreeFile inum f) ]] *
+               [[[ (DFData f) ::: (Fd * off |-> vs) ]]] *     
+               ([[ isError ok ]] \/
+                [[ ok = OK tt ]] * [[ can_access caller (DFOwner f) ]]))%pred d); simpl ;auto.
+    pred_apply; cancel.
+    or_l; cancel.
+    eauto.
+    or_r; cancel.
+    eauto.
+    inv_exec'' H7; simpl; auto.
+    eassign (fun (_:taggedmem) (_: domainmem) (_:rawdisk) => True); simpl;
+      intros mx Hmx; simpl; auto.
+  }
+  simpl in *; clear Hspec; cleanup; split_ors; cleanup; try congruence.
+  eapply exec_same_except_finished in H0; eauto; cleanup.
+  unfold pair_args_helper in *; simpl in *.
+  apply sep_star_or_distr in H5; apply pimpl_or_apply in H5;
+    split_ors; destruct_lift H5; cleanup.
+  inversion H9.
+  {
+    Transparent LOG.commit_ro LOG.abort.
+    unfold LOG.abort in *.
+    repeat inv_exec_perm.
+    do 4 eexists; split.
+    econstructor; eauto.
+    inversion H20; subst.
+    simpl; rewrite <- app_nil_l; repeat econstructor; eauto.
+    repeat split; simpl; eauto.
+    destruct (tag_dec tag (DFOwner f)); subst; intuition.
+    eapply same_except_to_equivalent_for; eauto.
+    destruct (tag_dec tag (DFOwner f)); subst; intuition.
+    eapply blockmem_same_except_to_equivalent_for; eauto.
+  }
+  {
+    (*inversion H9; subst.*)
+    Transparent LOG.commit_ro LOG.abort.
+    unfold LOG.commit_ro in *.
+    repeat inv_exec_perm.
+    inversion H22; subst.
+    specialize (H6 x8) as Hx; split_ors; cleanup; try congruence.
+    pose proof (@DIRTREE.dwrite_ok fsxp inum off x8 x8_1 caller) as Hspec.
+    specialize (Hspec _ (fun r => Ret r)).
+    unfold corr2 in *.
+    edestruct Hspec with (d:= x9).
+    Opaque DIRTREE.dwrite.
+    2: repeat econstructor; eauto.
+    {
+      repeat eexists; pred_apply; norm.
+      unfold stars; simpl.
+      erewrite LOG.rep_blockmem_subset. cancel.
+      eauto.
+      intuition eauto.
+      apply Mem.upd_eq; eauto.
+      simpl; auto.
+      destruct_lift H2.
+      inv_exec'' H12.
+      do 3 eexists; left; repeat eexists; eauto.
+      eassign (fun (_:rawdisk) (_:taggedmem) (_: domainmem) (_: BFILE.memstate) => True); simpl ;auto.
+      inv_exec'' H12; simpl; auto.
+      eassign (fun (_:taggedmem) (_: domainmem) (_:rawdisk) => True); simpl;
+        intros mx Hmx; simpl; auto.
+    }
+    simpl in *; clear H2 Hspec.
+    eapply exec_same_except_finished with (bm':=(Mem.upd x2 x8 (S inum, data1))) in H7;
+    eauto; cleanup.
+    do 4 eexists; split.
+    repeat econstructor; eauto.
+    simpl; repeat econstructor; eauto.
+    repeat split; simpl; eauto.
+    destruct (tag_dec tag (DFOwner f)); subst; intuition.
+    eapply same_except_to_equivalent_for; eauto.
+    destruct (tag_dec tag (DFOwner f)); subst; intuition.
+    eapply blockmem_same_except_to_equivalent_for; eauto.
+    eapply blockmem_same_except_upd_same; eauto.
+    unfold rep in H8; destruct_lift H8.
+    erewrite owner_match; eauto.
+    2: pred_apply' H2; cancel.
+    2: pred_apply; cancel.
+    denote tree_pred as Htp; erewrite subtree_extract in Htp; eauto.
+    unfold tree_pred in Htp; destruct_lift Htp.    
+    denote BFILE.rep as Hbf; unfold BFILE.rep in Hbf; destruct_lift Hbf.
+    denote listmatch as Hlm;
+       erewrite listmatch_length_pimpl in Hlm;
+      erewrite listmatch_isolate with (i:=inum) in Hlm.
+    unfold BFILE.file_match in Hlm.
+    destruct_lift Hlm.
+    denote INODE.rep as Hbf; unfold INODE.rep in Hbf; destruct_lift Hbf.
+    rewrite H32; apply H37.
+    rewrite <- H30.
+    eapply list2nmem_ptsto_bound; eauto; pred_apply; cancel.
+    eapply list2nmem_ptsto_bound; eauto; pred_apply; cancel.
+    destruct_lift Hlm.
+    rewrite <- H30; eapply list2nmem_ptsto_bound; eauto; pred_apply; cancel.
+  }
+  congruence.
+  apply same_except_refl.
+  apply blockmem_same_except_refl.
+Qed.
+
+
